Defined instr_size_1RealAsm semantic and pass to it

x86/RealAsm.v
@@ -15,751 +15,6 @@ Require Import Events.
 Require Import Values.
 Require Import Conventions1.
 Require Import SSAsm AsmFacts AsmRegs.
-(*
-Section WFASM.
-
-  Fixpoint in_builtin_arg (b: builtin_arg preg) (r: preg) :=
-    match b with
-    | BA x => if preg_eq r x then True else False
-    | BA_splitlong ba1 ba2 => in_builtin_arg ba1 r \/ in_builtin_arg ba2 r
-    | BA_addptr ba1 ba2 => in_builtin_arg ba1 r \/ in_builtin_arg ba2 r
-    | _ => False
-    end.
-
-  Inductive is_alloc : instruction -> Prop :=
-    is_alloc_intro sz ora olink:
-      is_alloc (Pallocframe sz ora olink).
-
-  Definition make_palloc f  : instruction :=
-    let sz := fn_stacksize f in
-    (Pallocframe sz (Ptrofs.sub (Ptrofs.repr (align sz 8)) (Ptrofs.repr (size_chunk Mptr))) (fn_ofs_link f)).
-
-  Lemma make_palloc_is_alloc:
-    forall f,
-      is_alloc (make_palloc f).
-  Proof. constructor. Qed.
-
-  Inductive is_free : instruction -> Prop :=
-    is_free_intro sz ora olink:
-      is_free (Pfreeframe sz ora olink).
-
-  Lemma is_free_dec:
-    forall i,
-      {is_free i} + {~ is_free i}.
-  Proof.
-    destruct i; try now (right; intro A; inv A).
-    left. econstructor; eauto.
-  Defined.
-  Inductive is_jmp: instruction -> Prop :=
-  | is_jmps_intro: forall i sg, is_jmp (Pjmp_s i sg)
-  | is_jmpr_intro: forall ir sg, is_jmp (Pjmp_r ir sg).
-
-
-  Inductive intermediate_instruction : instruction -> Prop :=
-  | ii_alloc i: is_alloc i -> intermediate_instruction i
-  | ii_jmp i: i = Pret \/ is_jmp i -> intermediate_instruction i.
-
-  Record wf_asm_function (f: function): Prop :=
-    {
-
-      wf_asm_alloc_only_at_beginning:
-        forall o sz ora olink,
-          find_instr o (fn_code f) = Some (Pallocframe sz ora olink) ->
-          o = 0;
-
-      wf_asm_alloc_at_beginning:
-        find_instr 0 (fn_code f) = Some (make_palloc f);
-
-      wf_asm_after_freeframe:
-        forall i o,
-          find_instr (Ptrofs.unsigned o) (fn_code f) = Some i ->
-          is_free i ->
-          exists i' ,
-            find_instr (Ptrofs.unsigned (Ptrofs.add o (Ptrofs.one))) (fn_code f) = Some i' /\
-            (i' = Pret \/ is_jmp i' );
-
-      wf_asm_ret_jmp_comes_after_freeframe:
-        forall i o,
-          find_instr (Ptrofs.unsigned o) (fn_code f) = Some i ->
-          i = Pret \/ is_jmp i ->
-          exists o' ifree,
-            find_instr (Ptrofs.unsigned o') (fn_code f) = Some ifree /\
-            is_free ifree /\
-            Ptrofs.unsigned o' + 1 = Ptrofs.unsigned o;
-
-      wf_asm_code_bounded:
-        0 <= code_size (fn_code f) <= Ptrofs.max_unsigned;
-
-      wf_asm_builtin_not_PC:
-        forall o ef args res,
-          find_instr o (fn_code f) = Some (Pbuiltin ef args res) ->
-          ~ in_builtin_res res PC /\
-          ~ in_builtin_res res RSP
-          /\ Forall (fun arg : builtin_arg preg => ~ in_builtin_arg arg RA) args;
-
-      wf_asm_jmp_no_rsp:
-        forall o (r: ireg) sg,
-          find_instr o (fn_code f) = Some (Pjmp_r r sg) ->
-          r <> RSP;
-
-      wf_asm_call_no_rsp:
-        forall o (r: ireg) sg,
-          find_instr o (fn_code f) = Some (Pcall_r r sg) ->
-          r <> RSP;
-
-      wf_asm_free_spec:
-        forall o sz ora olink,
-          find_instr o (fn_code f) = Some (Pfreeframe sz ora olink) ->
-          sz = fn_stacksize f /\ ora = Ptrofs.sub (Ptrofs.repr (align sz 8)) (Ptrofs.repr (size_chunk Mptr));
-
-      wf_allocframe_repr:
-        forall o sz ora olink,
-          find_instr o (fn_code f) = Some (Pallocframe sz ora olink) ->
-          align sz 8 - size_chunk Mptr =
-          Ptrofs.unsigned (Ptrofs.sub (Ptrofs.repr (align sz 8)) (Ptrofs.repr (size_chunk Mptr)));
-
-      wf_freeframe_repr:
-        forall o sz ora olink,
-          find_instr o (fn_code f) = Some (Pfreeframe sz ora olink) ->
-          Ptrofs.repr (align sz 8 - size_chunk Mptr) = Ptrofs.sub (Ptrofs.repr (align sz 8)) (Ptrofs.repr (size_chunk Mptr));
-    }.
-
-  Definition is_make_palloc a f :=  a = make_palloc f /\
-                                    align (fn_stacksize f) 8 - size_chunk Mptr =
-                                    Ptrofs.unsigned (Ptrofs.sub (Ptrofs.repr (align (fn_stacksize f) 8)) (Ptrofs.repr (size_chunk Mptr))).
-(*
-  Lemma pair_eq: forall {A B}
-                   (Adec: forall (a b: A), {a = b} + {a <> b})
-                   (Bdec: forall (a b: B), {a = b} + {a <> b}),
-      forall (a b: A * B), {a = b} + {a <> b}.
-  Proof.
-    intros.
-    destruct a, b.
-    destruct (Adec a a0), (Bdec b b0); subst;
-      first [ now (right; inversion 1; congruence)
-            | left; reflexivity ].
-  Defined.
-*)
-  Definition pallocframe_dec s s' o o' l l':
-    {Pallocframe s o l= Pallocframe s' o' l'} + {Pallocframe s o l <> Pallocframe s' o' l'}.
-  Proof.
-    destruct (zeq s s'); subst. 2: (now right; inversion 1).
-    destruct (Ptrofs.eq_dec o o'); subst. 2: (now right; inversion 1).
-    destruct (Ptrofs.eq_dec l l'); subst. 2: (now right; inversion 1).
-    left; reflexivity.
-  Defined.
-
-  Lemma and_dec: forall {A B: Prop},
-      { A } + { ~ A } ->
-      { B } + { ~ B } ->
-      { A /\ B } + { ~ (A /\ B) }.
-  Proof.
-    intros. destruct H, H0; [left|right|right|right]; intuition.
-  Qed.
-
-  Definition is_make_palloc_dec a f : { is_make_palloc a f } + { ~ is_make_palloc a f }.
-  Proof.
-    unfold is_make_palloc, make_palloc.
-    destruct a; try (now right; inversion 1).
-    apply and_dec.
-    apply pallocframe_dec.
-    apply zeq.
-  Defined.
-
-  Definition check_ret_or_jmp roj :=
-    match roj with
-    | Pret |Pjmp_r _ _ | Pjmp_s _ _=> true
-    | _ => false
-    end.
-
-  Definition valid_ret_or_jmp roj :=
-    match roj with
-    | Pjmp_r r _ =>  negb (preg_eq r RSP)
-    | _ => true
-    end.
-
-  Definition check_free f sz ora :=
-      sz = fn_stacksize f /\ ora = Ptrofs.sub (Ptrofs.repr (align sz 8)) (Ptrofs.repr (size_chunk Mptr)) /\
-      Ptrofs.repr (align sz 8 - size_chunk Mptr) = Ptrofs.sub (Ptrofs.repr (align sz 8)) (Ptrofs.repr (size_chunk Mptr)).
-
-  Definition check_free_dec f sz ora : { check_free f sz ora } + { ~ check_free f sz ora }.
-  Proof.
-    unfold check_free.
-    apply and_dec. 2: apply and_dec.
-    apply zeq. apply Ptrofs.eq_dec. apply Ptrofs.eq_dec.
-  Defined.
-
-  Definition check_builtin args res :=
-    ~ in_builtin_res res PC /\
-    ~ in_builtin_res res RSP
-    /\ Forall (fun arg : builtin_arg preg => ~ in_builtin_arg arg RA) args.
-
-  Lemma not_in_builtin_res_dec res r:
-    {~ in_builtin_res res r} + {~ ~ in_builtin_res res r}.
-  Proof.
-    induction res; simpl.
-    destruct (preg_eq x r); subst; intuition. left; inversion 1.
-    destruct IHres1, IHres2; try (right; now intuition). left. intuition congruence.
-  Qed.
-
-
-  Lemma not_in_builtin_arg_dec arg r:
-    {~ in_builtin_arg arg r} + {~ ~ in_builtin_arg arg r}.
-  Proof.
-    induction arg; simpl; try (try destr; left; now inversion 1).
-    destruct IHarg1, IHarg2; try (right; now intuition). left. intuition congruence.
-    destruct IHarg1, IHarg2; try (right; now intuition). left. intuition congruence.
-  Qed.
-
-  Definition check_builtin_dec args res: {check_builtin args res} + { ~ check_builtin args res}.
-  Proof.
-    unfold check_builtin.
-    repeat apply and_dec.
-    apply not_in_builtin_res_dec.
-    apply not_in_builtin_res_dec.
-    apply Forall_dec. intros.
-    apply not_in_builtin_arg_dec.
-  Defined.
-
-  Lemma find_instr_bound:
-    forall c o i,
-      find_instr o c = Some i ->
-      o + 1 <= code_size c.
-  Proof.
-    induction c; simpl; intros; eauto. congruence.
-    destr_in H. inv H. generalize (code_size_non_neg c). lia.
-    apply IHc in H. lia.
-  Qed.
-
-  Lemma find_instr_pos_positive:
-        forall c o i,
-          find_instr o c = Some i ->
-          0 <= o.
-   Proof.
-     induction c; intros; simpl; inv H. destr_in H1. lia.
-     eapply IHc in H1. lia.
-   Qed.
-
-  Lemma instr_size_repr : 0 <= 1 <= Ptrofs.max_unsigned.
-  Proof.
-    vm_compute. split; congruence.
-  Qed.
-
-  Lemma code_bounded_repr':
-    forall c
-      (RNG: 0 <= code_size c <= Ptrofs.max_unsigned)
-      i o
-      (FI: find_instr o c = Some i)
-      sz
-      (LE: 0 <= sz <= 1),
-      Ptrofs.unsigned (Ptrofs.add (Ptrofs.repr o) (Ptrofs.repr sz)) = o + sz.
-  Proof.
-    intros.
-    unfold Ptrofs.add.
-    rewrite (Ptrofs.unsigned_repr sz). 2: generalize (instr_size_repr); lia.
-    generalize (find_instr_bound _ _ _ FI) (find_instr_pos_positive _ _ _ FI). intros.
-    rewrite (Ptrofs.unsigned_repr o) by lia.
-    apply Ptrofs.unsigned_repr; lia.
-  Qed.
-
-  Lemma code_bounded_repr:
-    forall c
-      (RNG: 0 <= code_size c <= Ptrofs.max_unsigned)
-      i o
-      (FI: find_instr (Ptrofs.unsigned o) c = Some i)
-      sz
-      (LE: 0 <= sz <= instr_size i),
-      Ptrofs.unsigned (Ptrofs.add o (Ptrofs.repr sz)) = Ptrofs.unsigned o + sz.
-  Proof.
-    intros.
-    erewrite <- code_bounded_repr'; eauto.
-    unfold Ptrofs.add.
-    rewrite Ptrofs.repr_unsigned. reflexivity.
-  Qed.
-
-  Lemma wf_asm_pc_repr' : forall f : function,
-       wf_asm_function f ->
-       forall (i : instruction) (o : ptrofs),
-       find_instr (Ptrofs.unsigned o) (fn_code f) = Some i ->
-       forall sz : Z, 0 <= sz <= instr_size i ->
-       Ptrofs.unsigned (Ptrofs.add o (Ptrofs.repr sz)) = Ptrofs.unsigned o + sz.
-  Proof.
-    intros; eapply code_bounded_repr; eauto.
-    apply wf_asm_code_bounded; eauto.
-  Qed.
-
-  Fixpoint check_asm_body (f: function) (next_roj: bool) (r: code) : bool :=
-    match r with
-    | nil => negb next_roj
-    | i :: r =>
-      let roj := proj_sumbool (is_free_dec i) in
-      check_asm_body f roj r &&
-      if next_roj then check_ret_or_jmp i && valid_ret_or_jmp i
-      else
-        negb (check_ret_or_jmp i) &&
-        match i with
-        | Pfreeframe sz ora olink =>     (* after a free, ret or jmp *)
-          check_free_dec f sz ora
-        | Pallocframe _ _ _ => false (* no alloc in body *)
-        | Pcall_r r sg => negb (preg_eq r RSP)
-        | Pbuiltin _ args res => check_builtin_dec args res
-        | _ => true
-      end
-    end.
-
-  Definition wf_asm_function_check (f: function) : bool :=
-    match fn_code f with
-    | nil => false
-    | a::r => is_make_palloc_dec a f && check_asm_body f false r
-    end && zle (code_size (fn_code f)) Ptrofs.max_unsigned.
-
-  Lemma check_asm_body_no_alloc:
-    forall f c b i,
-      check_asm_body f b c = true ->
-      In i c ->
-      ~ is_alloc i.
-  Proof.
-    induction c; simpl; intros. easy.
-    intro IA. inv IA.
-    assert (exists b, check_asm_body f b c = true).
-    {
-      eexists. refine (proj1 _); apply andb_true_iff; eauto.
-    }
-    destruct H1.
-    destruct H0. subst. simpl in *.
-    apply andb_true_iff in H. destruct H. destr_in H0.
-    eapply IHc in H0; eauto. apply H0; constructor.
-  Qed.
-
-  Lemma find_instr_app:
-    forall a o b,
-      0 <= o ->
-      find_instr (o + code_size a) (a ++ b) = find_instr o b.
-  Proof.
-    induction a; simpl; intros; eauto.
-    f_equal. lia.
-    rewrite pred_dec_false.
-    rewrite <- (IHa o b). f_equal. unfold instr_size. lia. lia.
-    generalize (code_size_non_neg a0). unfold instr_size. lia.
-  Qed.
-
-  Lemma find_instr_app':
-    forall a o b,
-      code_size a <= o ->
-      find_instr o (a ++ b) = find_instr (o - code_size a) b.
-  Proof.
-    intros.
-    rewrite <- (find_instr_app a _ b). f_equal. lia. lia.
-  Qed.
-
-  Lemma find_instr_split:
-    forall c o i,
-      find_instr o c = Some i ->
-      exists a b, c = a ++ i :: b /\ o = code_size a.
-  Proof.
-    induction c; simpl; intros; eauto. congruence.
-    destr_in H. inv H. eexists nil, c; simpl. split; auto.
-    edestruct IHc as (aa & b & EQ & SZ). apply H. subst.
-    exists (a::aa), b; simpl; split; auto.
-    generalize (instr_size_positive a). lia.
-  Qed.
-
-  Lemma find_instr_app_pres: forall f1 f2 ofs i,
-      find_instr ofs f1 = Some i ->
-      find_instr ofs (f1 ++ f2) = Some i.
-  Proof.
-    induction f1 as [|i1 f1].
-    - cbn. intros; congruence.
-    - cbn. intros f2 i FI.
-      destr. eauto.
-  Qed.
-
-  Lemma code_size_app:
-    forall c1 c2,
-      code_size (c1 ++ c2) = code_size c1 + code_size c2.
-  Proof.
-    induction c1; simpl; intros; eauto. rewrite IHc1. lia.
-  Qed.
-
-  Lemma check_asm_body_after_free:
-    forall f a i b roj,
-      check_asm_body f roj (a ++ i :: b) = true ->
-      is_free i ->
-      check_asm_body f true b = true.
-  Proof.
-    induction a; simpl; intros; eauto.
-    apply andb_true_iff in H. destruct H as (H & _).
-    inv H0. simpl in *. auto.
-    apply andb_true_iff in H. destruct H as (H & B).
-    destruct (is_free_dec a); simpl in *. inv i0.
-    eapply IHa; eauto.
-    eapply IHa; eauto.
-  Qed.
-
-
-  Lemma check_asm_body_call:
-    forall f c b r sg,
-      check_asm_body f b c = true ->
-      In (Pcall_r r sg) c ->
-      r <> RSP.
-  Proof.
-    induction c; simpl; intros. easy.
-    assert (exists b, check_asm_body f b c = true).
-    {
-      eexists. refine (proj1 _); apply andb_true_iff; eauto.
-    }
-    apply andb_true_iff in H. destruct H. destruct H1. destruct H0; eauto. subst. simpl in *.
-    destr_in H2; simpl in *.
-    unfold proj_sumbool in H2; destr_in H2. simpl in H2. congruence.
-  Qed.
-
-  Lemma check_asm_body_free:
-    forall f c b sz ora olink,
-      check_asm_body f b c = true ->
-      In (Pfreeframe sz ora olink) c ->
-      check_free f sz ora.
-  Proof.
-    induction c; simpl; intros. easy.
-    assert (exists b, check_asm_body f b c = true).
-    {
-      eexists. refine (proj1 _); apply andb_true_iff; eauto.
-    }
-    apply andb_true_iff in H. destruct H. destruct H1. destruct H0; eauto. subst. simpl in *.
-    destr_in H2; simpl in *.
-    unfold proj_sumbool in H2; destr_in H2.
-  Qed.
-
-  Lemma check_asm_body_before_roj:
-    forall f a i b roj,
-      check_asm_body f roj (a ++ i :: b) = true ->
-      i = Pret \/ is_jmp i ->
-      (a = nil /\ roj = true) \/ exists a0 i0, a = a0 ++ i0 :: nil /\ is_free i0.
-  Proof.
-    induction a; simpl; intros; eauto.
-    - apply andb_true_iff in H. destruct H as (A & B).
-      destruct H0 as [ROJ|ROJ]; inv ROJ; simpl in *. destr_in B.
-      destruct roj. auto. congruence. destr_in B.
-    - apply andb_true_iff in H. destruct H as (A & B).
-      destruct (is_free_dec a); simpl in *. inv i0.
-      + simpl in *. destr_in B. right.
-        destruct a0. clear IHa. simpl in *.
-        eexists nil, _. split. simpl. eauto. constructor.
-        edestruct IHa as [ROJ|(a1 & i1 & EQ & IFR)]; eauto.
-        destruct ROJ; congruence. rewrite EQ.
-        eexists (_ :: a1), i1; split. simpl. reflexivity. auto.
-      + edestruct IHa as [ROJ|(a1 & i1 & EQ & IFR)]; eauto.
-        destruct ROJ; congruence. subst. right.
-        eexists (_ :: a1), i1; split. simpl. reflexivity. auto.
-  Qed.
-
-  Lemma check_asm_body_builtin:
-    forall f c b ef args res,
-      check_asm_body f b c = true ->
-      In (Pbuiltin ef args res) c ->
-      check_builtin args res.
-  Proof.
-    induction c; simpl; intros. easy.
-    assert (exists b, check_asm_body f b c = true).
-    {
-      eexists. refine (proj1 _); apply andb_true_iff; eauto.
-    }
-    destruct H1.
-    destruct H0. subst. simpl in *.
-    apply andb_true_iff in H. destruct H. destr_in H0.
-    unfold proj_sumbool in H0; destr_in H0.
-    eapply IHc in H0; eauto.
-  Qed.
-
-  Lemma check_asm_body_jmp:
-    forall f c b r sg,
-      check_asm_body f b c = true ->
-      In (Pjmp_r  r sg) c ->
-      r <> RSP.
-  Proof.
-    induction c; simpl; intros. easy.
-    assert (exists b, check_asm_body f b c = true).
-    {
-      eexists. refine (proj1 _); apply andb_true_iff; eauto.
-    }
-    apply andb_true_iff in H. destruct H. destruct H1. destruct H0; eauto. subst. simpl in *.
-    destr_in H2; simpl in *.
-    unfold proj_sumbool in H2; destr_in H2. simpl in H2. congruence.
-  Qed.
-
-  Lemma wf_asm_function_check_correct f:
-    wf_asm_function_check f = true ->
-    wf_asm_function f.
-  Proof.
-    unfold wf_asm_function_check. destr. simpl. congruence.
-    rewrite ! andb_true_iff. intros ((A & B) & C).
-    unfold proj_sumbool in A, C. destr_in A; destr_in C.
-    clear A C. rename Heqc into CODE. rename l into SIZE.
-    constructor.
-    - rewrite CODE. simpl. intros. destr_in H.
-      apply Asmgenproof0.find_instr_in in H.
-      eapply check_asm_body_no_alloc in H; eauto. contradict H. constructor.
-    - rewrite CODE; simpl. clear - i0. destruct i0 as (A & B). subst. reflexivity.
-    - destruct i0 as (i0 & _). subst. rewrite CODE. simpl.
-      intros. destr_in H. inv H. inv H0.
-      simpl in SIZE.
-      rewrite pred_dec_false. unfold Ptrofs.one.
-      replace (Ptrofs.unsigned (Ptrofs.add o (Ptrofs.repr 1)) - 1)
-        with (Ptrofs.unsigned (Ptrofs.add (Ptrofs.repr (Ptrofs.unsigned o - 1)) (Ptrofs.repr 1))).
-      revert H.
-      generalize (Ptrofs.unsigned o - 1).
-      intros.
-      edestruct find_instr_split as (a & b & EQ & SZ). apply H. subst.
-      rewrite find_instr_app'.
-      simpl. rewrite pred_dec_false.
-      eapply check_asm_body_after_free in B; eauto.
-      destruct b; simpl in B. congruence. simpl. rewrite pred_dec_true. eexists; split; eauto.
-      apply andb_true_iff in B. destruct B as (B & CHK).
-      unfold check_ret_or_jmp in CHK. apply andb_true_iff in CHK. destruct CHK as (CHK & _). destr_in CHK; try (right; constructor).
-      unfold Ptrofs.add.
-      rewrite (Ptrofs.unsigned_repr (code_size a) ).
-      setoid_rewrite (Ptrofs.unsigned_repr 1).
-      rewrite Ptrofs.unsigned_repr. lia.
-      simpl in SIZE. rewrite code_size_app in SIZE. simpl in SIZE.
-      generalize (code_size_non_neg a) (instr_size_positive i) (instr_size_positive i0) (code_size_non_neg b)
-                 (instr_size_positive (make_palloc f)). lia.
-      vm_compute. split; congruence.
-      simpl in SIZE. rewrite code_size_app in SIZE. simpl in SIZE.
-      generalize (code_size_non_neg a) (instr_size_positive i) (instr_size_positive i0) (code_size_non_neg b)
-                 (instr_size_positive (make_palloc f)). lia.
-      unfold Ptrofs.add.
-      rewrite (Ptrofs.unsigned_repr (code_size a)).
-      rewrite (Ptrofs.unsigned_repr 1).
-      rewrite Ptrofs.unsigned_repr. generalize (instr_size_positive i); lia.
-      simpl in SIZE. rewrite code_size_app in SIZE. simpl in SIZE.
-      generalize (code_size_non_neg a) (instr_size_positive i) (code_size_non_neg b)
-                 (instr_size_positive (make_palloc f)). lia.
-      vm_compute. split; congruence.
-      simpl in SIZE. rewrite code_size_app in SIZE. simpl in SIZE.
-      generalize (code_size_non_neg a) (instr_size_positive i) (code_size_non_neg b)
-                 (instr_size_positive (make_palloc f)). simpl in SIZE. lia.
-      unfold Ptrofs.add.
-      rewrite (Ptrofs.unsigned_repr (code_size a)).
-      rewrite (Ptrofs.unsigned_repr 1).
-      rewrite Ptrofs.unsigned_repr. generalize (instr_size_positive i); lia.
-      simpl in SIZE. rewrite code_size_app in SIZE. simpl in SIZE.
-      generalize (code_size_non_neg a) (instr_size_positive i) (code_size_non_neg b)
-                 (instr_size_positive (make_palloc f)). lia.
-      vm_compute. split; congruence.
-      simpl in SIZE. rewrite code_size_app in SIZE. simpl in SIZE.
-      generalize (code_size_non_neg a) (instr_size_positive i) (code_size_non_neg b)
-                 (instr_size_positive (make_palloc f)). lia.
-      unfold Ptrofs.add.
-      rewrite (Ptrofs.unsigned_repr 1).
-      rewrite (Ptrofs.unsigned_repr (Ptrofs.unsigned o - _)).
-      rewrite ! Ptrofs.unsigned_repr. lia.
-      generalize (find_instr_bound _ _ _ H) (find_instr_pos_positive _ _ _ H).
-      generalize (instr_size_positive i)
-                 (instr_size_positive (make_palloc f)). lia.
-      generalize (find_instr_bound _ _ _ H) (find_instr_pos_positive _ _ _ H).
-      generalize (instr_size_positive i)
-                 (instr_size_positive (make_palloc f)). lia.
-      generalize (find_instr_bound _ _ _ H) (find_instr_pos_positive _ _ _ H).
-      generalize (instr_size_positive i)
-                 (instr_size_positive (make_palloc f)). lia.
-      vm_compute. split; congruence.
-      unfold Ptrofs.add. unfold Ptrofs.one.
-      rewrite (Ptrofs.unsigned_repr 1).
-      rewrite Ptrofs.unsigned_repr.
-      generalize (Ptrofs.unsigned_range o) (instr_size_positive i); lia.
-      generalize (find_instr_bound _ _ _ H) (find_instr_pos_positive _ _ _ H).
-      generalize (instr_size_positive i)
-                 (instr_size_positive (make_palloc f)). lia.
-      vm_compute. split; congruence.
-    - destruct i0 as (i0 & _). subst. rewrite CODE. simpl.
-      intros i o FI ROJ.
-      destr_in FI. inv FI. destruct ROJ as [ROJ|ROJ]; inv ROJ.
-      edestruct find_instr_split as (a & b & EQ & SZ). apply FI. subst.
-      destruct (check_asm_body_before_roj _ _ _ _ _ B ROJ) as [(NIL & ROJFALSE)|(a0 & i0 & EQ & IFR)]. congruence.
-      subst.
-      exists (Ptrofs.sub o (Ptrofs.repr (instr_size i0))), i0.
-      rewrite pred_dec_false.
-      replace (Ptrofs.unsigned (Ptrofs.sub o (Ptrofs.repr (instr_size i0))) - 1)
-        with (0 + code_size a0). rewrite app_ass.
-      rewrite find_instr_app. simpl. split; auto. split. auto.
-      unfold Ptrofs.sub.
-      rewrite (Ptrofs.unsigned_repr _ (instr_size_repr i0)).
-      rewrite Ptrofs.unsigned_repr. unfold instr_size. lia.
-      generalize (find_instr_bound _ _ _ FI) (find_instr_pos_positive _ _ _ FI). intros.
-      simpl in *. rewrite ! code_size_app in *. simpl in *.
-      generalize (code_size_non_neg a0) (instr_size_positive i) (instr_size_positive i0) (code_size_non_neg b)
-                 (instr_size_positive (make_palloc f)). lia.
-      lia.
-      unfold Ptrofs.sub.
-      rewrite (Ptrofs.unsigned_repr _ (instr_size_repr i0)).
-      rewrite Ptrofs.unsigned_repr.
-      simpl in *. rewrite ! code_size_app in *. simpl in *. lia.
-      generalize (find_instr_bound _ _ _ FI) (find_instr_pos_positive _ _ _ FI). intros.
-      simpl in *. rewrite ! code_size_app in *. simpl in *.
-      generalize (code_size_non_neg a0) (instr_size_positive i) (instr_size_positive i0) (code_size_non_neg b)
-                 (instr_size_positive (make_palloc f)). lia.
-      unfold Ptrofs.sub.
-      rewrite (Ptrofs.unsigned_repr _ (instr_size_repr i0)).
-      rewrite Ptrofs.unsigned_repr.
-      simpl in *. rewrite ! code_size_app in *. simpl in *.
-      generalize (find_instr_bound _ _ _ FI) (find_instr_pos_positive _ _ _ FI). intros.
-      simpl in *. rewrite ! code_size_app in *. simpl in *.
-      generalize (code_size_non_neg a0) (instr_size_positive i) (instr_size_positive i0) (code_size_non_neg b)
-                 (instr_size_positive (make_palloc f)). lia.
-      generalize (find_instr_bound _ _ _ FI) (find_instr_pos_positive _ _ _ FI). intros.
-      simpl in *. rewrite ! code_size_app in *. simpl in *.
-      generalize (code_size_non_neg a0) (instr_size_positive i) (instr_size_positive i0) (code_size_non_neg b)
-                 (instr_size_positive (make_palloc f)). lia.
-    - rewrite CODE; split; auto.
-      generalize (code_size_non_neg (i::c)). lia.
-    - destruct i0 as (i0 & _). subst. rewrite CODE. simpl.
-      intros o ef args res FI.
-      destr_in FI. inv FI.
-      apply Asmgenproof0.find_instr_in in FI.
-      eapply check_asm_body_builtin in FI; eauto.
-    - destruct i0 as (i0 & _). subst. rewrite CODE. simpl.
-      intros o r sg FI.
-      destr_in FI. inv FI.
-      apply Asmgenproof0.find_instr_in in FI.
-      eapply check_asm_body_jmp in FI; eauto.
-    - destruct i0 as (i0 & _). subst. rewrite CODE. simpl.
-      intros o r sg FI.
-      destr_in FI. inv FI.
-      apply Asmgenproof0.find_instr_in in FI.
-      eapply check_asm_body_call in FI; eauto.
-    - destruct i0 as (i0 & _). subst. rewrite CODE. simpl.
-      intros o sz ora olink FI.
-      destr_in FI. inv FI.
-      apply Asmgenproof0.find_instr_in in FI.
-      edestruct check_asm_body_free as (A & BB & C); subst; eauto.
-    - destruct i0 as (i0 & PA). subst. rewrite CODE. simpl.
-      intros o sz pubrange ora FI.
-      destr_in FI. inv FI; auto.
-      apply Asmgenproof0.find_instr_in in FI.
-      eapply check_asm_body_no_alloc in FI; eauto. contradict FI; constructor.
-    - destruct i0 as (i0 & _). subst. rewrite CODE. simpl.
-      intros o sz ora olink FI.
-      destr_in FI. inv FI.
-      apply Asmgenproof0.find_instr_in in FI.
-      edestruct check_asm_body_free as (A & BB & C); subst; eauto.
-  Qed.
-
-  Lemma wf_asm_pc_repr:
-    forall f (WF: wf_asm_function f) i o,
-      find_instr (Ptrofs.unsigned o) (fn_code f) = Some i ->
-      Ptrofs.unsigned (Ptrofs.add o (Ptrofs.repr (instr_size i))) = Ptrofs.unsigned o + instr_size i.
-  Proof.
-    intros; eapply wf_asm_pc_repr'; eauto. generalize (instr_size_positive i); lia.
-  Qed.
-
-  Lemma wf_asm_wf_allocframe:
-    forall f (WF: wf_asm_function f) o sz ora olink
-      (FI: find_instr o (fn_code f) = Some (Pallocframe sz ora olink)),
-      make_palloc f = Pallocframe sz ora olink.
-  Proof.
-    intros.
-    exploit wf_asm_alloc_only_at_beginning; eauto. intro; subst.
-    erewrite wf_asm_alloc_at_beginning in FI; eauto. inv FI; auto.
-  Qed.
-
-End WFASM.
-*)
-(*
-Section INSTR_SIZE.
-
-Definition instr_size (i:instruction) := 1%Z.
-
-Lemma instr_size_repr : forall i, 0<= instr_size i <= Ptrofs.max_unsigned.
-Proof.
-  intro. unfold instr_size. vm_compute. split; congruence.
-Qed.
-
-Lemma instr_size_positive :forall i, 0 < instr_size i.
-Proof.
-  intro. unfold instr_size. lia.
-Qed.
-
-Lemma code_size_non_neg: forall c, 0 <= code_size c.
-Proof.
-  intros. induction c; simpl. lia.
-  generalize (instr_size_positive a). lia.
-Qed.
-
-(** Looking up instructions in a code sequence by position. *)
-
-Fixpoint find_instr (pos: Z) (c: code) {struct c} : option instruction :=
-  match c with
-  | nil => None
-  | i :: il => if zeq pos 0 then Some i else find_instr (pos - instr_size i) il
-  end.
-
-Fixpoint label_pos (lbl: label) (pos: Z) (c: code) {struct c} : option Z :=
-  match c with
-  | nil => None
-  | instr :: c' =>
-    let nextpos := pos + instr_size instr in
-      if is_label lbl instr then Some nextpos else label_pos lbl nextpos c'
-  end.
-
-Lemma label_pos_rng:
-  forall lbl c pos z,
-    label_pos lbl pos c = Some z ->
-    0 <= pos ->
-    0 <= z - pos <= code_size c.
-Proof.
-  induction c; simpl; intros; eauto. congruence. repeat destr_in H.
-  generalize (code_size_non_neg c) (instr_size_positive a). lia.
-  apply IHc in H2.
-  generalize (instr_size_positive a); lia.
-  generalize (instr_size_positive a); lia.
-Qed.
-
-Lemma label_pos_repr:
-  forall lbl c pos z,
-    code_size c + pos <= Ptrofs.max_unsigned ->
-    0 <= pos ->
-    label_pos lbl pos c = Some z ->
-    Ptrofs.unsigned (Ptrofs.repr (z - pos)) = z - pos.
-Proof.
-  intros.
-  apply Ptrofs.unsigned_repr.
-  generalize (label_pos_rng _ _ _ _ H1 H0). lia.
-Qed.
-
-Lemma find_instr_ofs_pos:
-  forall c o i,
-    find_instr o c = Some i ->
-    0 <= o.
-Proof.
-  induction c; simpl; intros; repeat destr_in H.
-  lia. apply IHc in H1.
-  generalize (instr_size_positive a); lia.
-Qed.
-
-Lemma label_pos_spec:
-  forall lbl c pos z,
-    code_size c + pos <= Ptrofs.max_unsigned ->
-    0 <= pos ->
-    label_pos lbl pos c = Some z ->
-    find_instr ((z - pos) - instr_size (Plabel lbl)) c = Some (Plabel lbl).
-Proof.
-  induction c; simpl; intros; repeat destr_in H1.
-  destruct a; simpl in Heqb; try congruence. repeat destr_in Heqb.
-  apply pred_dec_true. generalize (instr_size_positive (Plabel l)). lia.
-  eapply IHc in H3.
-  2: lia.  2: generalize (instr_size_positive a); lia.
-  generalize (find_instr_ofs_pos _ _ _ H3). intro.
-  rewrite pred_dec_false.  2: generalize (instr_size_positive a); lia.
-  rewrite <- H3. f_equal. lia.
-Qed.
-
-Definition nextinstr (rs: regset) (sz:ptrofs) :=
-  rs#PC <- (Val.offset_ptr rs#PC sz).
-
-Definition nextinstr_nf (rs: regset) (sz:ptrofs) : regset :=
-  nextinstr (undef_regs (CR ZF :: CR CF :: CR PF :: CR SF :: CR OF :: nil) rs) sz.
-
-End INSTR_SIZE.
-*)
 
 (** * Operational Semantics with instr_size *)
 Section INSTRSIZE.
@@ -787,15 +42,28 @@ Fixpoint label_pos (lbl: label) (pos: Z) (c: code) {struct c} : option Z :=
       if is_label lbl instr then Some nextpos else label_pos lbl nextpos c'
   end.
 
+Section WITHGE.
+  Variable ge : Genv.t Asm.fundef unit.
+
 Definition nextinstr (rs: regset) (sz:ptrofs) :=
   rs#PC <- (Val.offset_ptr rs#PC sz).
 
 Definition nextinstr_nf (rs: regset) (sz:ptrofs) : regset :=
   nextinstr (undef_regs (CR ZF :: CR CF :: CR PF :: CR SF :: CR OF :: nil) rs) sz.
 
-
-Section WITHGE.
-  Variable ge : Genv.t Asm.fundef unit.
+Definition goto_label (f: function) (lbl: label) (rs: regset) (m: mem) :=
+  match label_pos lbl 0 (fn_code f) with
+  | None => Stuck
+  | Some pos =>
+      match rs#PC with
+      | Vptr b ofs =>
+        match Genv.find_funct_ptr ge b with
+        | Some _ => Next (rs#PC <- (Vptr b (Ptrofs.repr pos))) m
+        | None => Stuck
+        end
+      | _ => Stuck
+    end
+  end.
 
 (** Auxiliaries for memory accesses. *)
 
@@ -814,7 +82,7 @@ Definition exec_store (chunk: memory_chunk) (m: mem)
   | None => Stuck
   end.
 
-Definition exec_instr (f: function) (i: instruction) (rs: regset) (m: mem) : outcome :=
+Definition exec_instr_asm (f: function) (i: instruction) (rs: regset) (m: mem) : outcome :=
   let sz := Ptrofs.repr (instr_size i) in
   match i with
   (** Moves *)
@@ -1105,7 +373,7 @@ Definition exec_instr (f: function) (i: instruction) (rs: regset) (m: mem) : out
       Next (nextinstr_nf (rs#rd <- (Vsingle Float32.zero)) sz) m
   (** Branches and calls *)
   | Pjmp_l lbl =>
-      goto_label ge f lbl rs m
+      goto_label f lbl rs m
   | Pjmp_s id sg =>
     let addr := Genv.symbol_address ge id Ptrofs.zero in
     match Genv.find_funct ge addr with
@@ -1122,13 +390,13 @@ Definition exec_instr (f: function) (i: instruction) (rs: regset) (m: mem) : out
     end
   | Pjcc cond lbl =>
       match eval_testcond cond rs with
-      | Some true => goto_label ge f lbl rs m
+      | Some true => goto_label f lbl rs m
       | Some false => Next (nextinstr rs sz) m
       | None => Stuck
       end
   | Pjcc2 cond1 cond2 lbl =>
       match eval_testcond cond1 rs, eval_testcond cond2 rs with
-      | Some true, Some true => goto_label ge f lbl rs m
+      | Some true, Some true => goto_label f lbl rs m
       | Some _, Some _ => Next (nextinstr rs sz) m
       | _, _ => Stuck
       end
@@ -1137,7 +405,7 @@ Definition exec_instr (f: function) (i: instruction) (rs: regset) (m: mem) : out
       | Vint n =>
           match list_nth_z tbl (Int.unsigned n) with
           | None => Stuck
-          | Some lbl => goto_label ge f lbl (rs #RAX <- Vundef #RDX <- Vundef) m
+          | Some lbl => goto_label f lbl (rs #RAX <- Vundef #RDX <- Vundef) m
           end
       | _ => Stuck
       end
@@ -1267,7 +535,8 @@ Definition exec_instr (f: function) (i: instruction) (rs: regset) (m: mem) : out
   end.
 
 (* maybe useful to prove SSAsm -> RealAsm_1 *)
-(*  Definition exec_instr f i rs (m: mem) :=
+  Definition exec_instr f i rs (m: mem) :=
+    let isz := Ptrofs.repr (instr_size i) in
     match i with
     | Pallocframe sz ofs_ra ofs_link =>
       let aligned_sz := align sz 8 in
@@ -1276,11 +545,11 @@ Definition exec_instr (f: function) (i: instruction) (rs: regset) (m: mem) : out
       match Mem.storev Mptr m (Val.offset_ptr sp ofs_link) psp with
         |None => Stuck
         |Some m1 =>
-      Next (nextinstr (rs #RAX <- (Val.offset_ptr (rs RSP) (Ptrofs.repr (size_chunk Mptr))) #RSP <- sp)) m1
+      Next (nextinstr (rs #RAX <- (Val.offset_ptr (rs RSP) (Ptrofs.repr (size_chunk Mptr))) #RSP <- sp) isz) m1
       end
     | Pfreeframe sz ofs_ra ofs_link =>
       let sp := Val.offset_ptr (rs RSP) (Ptrofs.sub (Ptrofs.repr (align sz 8)) (Ptrofs.repr (size_chunk Mptr))) in
-      Next (nextinstr (rs#RSP <- sp)) m
+      Next (nextinstr (rs#RSP <- sp) isz) m
     | Pcall_s i sg =>
       let sp := Val.offset_ptr (rs RSP) (Ptrofs.neg (Ptrofs.repr (size_chunk Mptr))) in
       match Mem.storev Mptr m sp (Val.offset_ptr rs#PC Ptrofs.one) with
@@ -1308,9 +577,8 @@ Definition exec_instr (f: function) (i: instruction) (rs: regset) (m: mem) : out
                  #PC <- ra
                  #RA <- Vundef) m
       end
-    | _ => Asm.exec_instr ge f i rs m
+    | _ => exec_instr_asm f i rs m
     end.
-*)
 
   Inductive step  : state -> trace -> state -> Prop :=
   | exec_step_internal:
@@ -1371,298 +639,6 @@ Inductive initial_state (p: Asm.program): state -> Prop :=
 
 Definition semantics prog :=
   Semantics step (initial_state prog) final_state (Genv.globalenv prog).
-
-Definition rs_state s :=
-  let '(State rs _) := s in rs.
-Definition m_state s :=
-  let '(State _ m) := s in m.
-
-
-
-(* Syntactic or Semantic ? *)
-  Section INVARIANT.
-
-    Variable prog: Asm.program.
-    Let ge := Genv.globalenv prog.
-
-    Definition bstack := stkblock.
-
-    Definition rsp_ptr (s: state) : Prop :=
-      exists o, rs_state s RSP = Vptr bstack o /\ (align_chunk Mptr | Ptrofs.unsigned o).
-
-    Definition bstack_perm (s: state) : Prop :=
-      forall o k p,
-        Mem.perm (m_state s) bstack o k p ->
-        Mem.perm (m_state s) bstack o k Writable.
-
-    Definition stack_top_state (s: state) : Prop :=
-      exists tl st, Mem.stack(Mem.support (m_state s))= Node None (1%positive::nil) tl st.
-
-    Inductive real_asm_inv : state -> Prop :=
-    | real_asm_inv_intro:
-        forall s
-          (RSPPTR: rsp_ptr s)
-          (BSTACKPERM: bstack_perm s)
-          (STOP: stack_top_state s),
-          real_asm_inv s.
-
-    Lemma storev_perm :
-      forall m chunk addr v m', Mem.storev chunk m addr v = Some m' ->
-                           (forall b o k p, Mem.perm m' b o k p <-> Mem.perm m b o k p).
-      Proof.
-        intros. unfold Mem.storev in H. destr_in H. split.
-        eapply Mem.perm_store_2; eauto. eapply Mem.perm_store_1; eauto.
-      Qed.
-
-    Lemma real_initial_inv:
-      forall is,
-        initial_state prog is -> real_asm_inv is.
-    Proof.
-      intros. inv H.
-      apply Genv.init_mem_stack in H0 as STK.
-      constructor.
-      - red. simpl. unfold rs0; simpl_regs. eexists. split. reflexivity.
-        apply div_ptr_add.
-        apply div_unsigned_repr.
-        apply Z.divide_add_r. apply align_Mptr_stack_limit. apply align_Mptr_align8.
-        apply align_Mptr_modulus. unfold Ptrofs.neg. apply div_unsigned_repr.
-        apply Zdivide_opp_r.
-        apply div_unsigned_repr.
-        apply align_size_chunk_divides.
-        apply align_Mptr_modulus.
-        apply align_Mptr_modulus.
-        apply align_Mptr_modulus.
-      - exploit Mem.alloc_result; eauto. intro. subst.
-        unfold Mem.nextblock in H1. unfold Mem.fresh_block in H1.
-        rewrite STK in H1. destr_in H1. simpl in Heqp. inv Heqp.
-        red. unfold bstack. unfold stkblock. intros o k p.
-        repeat erewrite (storev_perm _ _ _ _ _ H2). eauto.
-        intro. exploit Mem.perm_alloc_3; eauto.
-        intro. exploit Mem.perm_alloc_2; eauto. simpl. intro. eapply Mem.perm_implies; eauto.
-        apply perm_F_any.
-      - red. simpl. apply Mem.stack_alloc in H1. rewrite STK in H1.
-        exists nil, None. simpl in H1. erewrite <- Mem.support_storev; eauto.
-Qed.
-
-    Lemma exec_instr_invar_same:
-      forall f i rs1 m1,
-        stk_unrelated_instr i = true ->
-        exec_instr ge f i rs1 m1 = SSAsm.exec_instr ge f i rs1 m1.
-    Proof.
-      intros f i rs1 m1 SI.
-      destruct i; simpl in SI; simpl; congruence.
-    Qed.
-(*
-    Inductive is_load_parent_pointer: instruction -> Prop :=
-    | ilpp_intro i z: is_load_parent_pointer (Pload_parent_pointer i z).
-
-    Lemma is_load_parent_pointer_dec i: { is_load_parent_pointer i } + { ~ is_load_parent_pointer i }.
-    Proof.
-      destruct i; first [ now (right; inversion 1) | left; econstructor ].
-    Defined.
-*)
-    Lemma exec_instr_invar_same':
-      forall f i rs1 m1,
-        stk_unrelated_instr i = true ->
-        Asm.exec_instr ge f i rs1 m1 = SSAsm.exec_instr ge f i rs1 m1.
-    Proof.
-      intros f i rs1 m1 SI.
-      destruct i; simpl in SI; simpl; try congruence.
-    Qed.
-
-    Lemma exec_instr_invar_inv:
-      forall f i rs1 m1 rs2 m2,
-        asm_instr_unchange_rsp i ->
-        stk_unrelated_instr i = true ->
-        exec_instr ge f i rs1 m1 = Next rs2 m2 ->
-        real_asm_inv (State rs1 m1) ->
-        real_asm_inv (State rs2 m2).
-    Proof.
-      intros f i rs1 m1 rs2 m2 NORSP INVAR EI RAI; inv RAI.
-     (* - constructor.
-        + red in RSPPTR; red.
-          simpl in *.
-          destruct RSPPTR as (o & EQ & AL).
-          red in NORSP.
-          exists o. split. exploit NORSP; eauto.
-          simpl_regs.
-          setoid_rewrite Pregmap.gsspec. destr. inv e. rewrite EQ.
-          simpl.
-          eexists; split; eauto. apply div_ptr_add. auto. apply div_unsigned_repr.
-          transitivity 8.
-          unfold Mptr. destr; simpl. exists 1; lia. exists 2; lia.
-          apply align_divides. lia.
-          apply align_Mptr_modulus.
-          apply align_Mptr_modulus.
-          eauto.
-        + red in BSTACKPERM; red. simpl in *. intros.
-          inv i0; simpl in EI; inv EI. eauto.
-        + red in STOP; red. simpl in *.
-          inv i0; simpl in EI; inv EI. eauto. *)
-      erewrite exec_instr_invar_same in EI; eauto.
-      erewrite <- exec_instr_invar_same' in EI; eauto.
-      exploit NORSP; eauto. intro EQ.
-      generalize (asm_prog_unchange_sup i INVAR _ _ _ _ _ _ EI). intros (A & B).
-      constructor.
-      + red in RSPPTR; red. simpl in *; rewrite <- EQ. eauto.
-      + red in BSTACKPERM; red. simpl in *. setoid_rewrite <- B. eauto.
-      + red in STOP; red; simpl in *. rewrite <- A; eauto.
-    Qed.
-
-    Lemma align_Mptr_sub:
-      forall o,
-        (align_chunk Mptr | Ptrofs.unsigned o) ->
-        (align_chunk Mptr | Ptrofs.unsigned (Ptrofs.add o (Ptrofs.neg (Ptrofs.repr (size_chunk Mptr))))).
-    Proof.
-      intros.
-      apply div_ptr_add; auto.
-      apply div_unsigned_repr.
-      apply Z.divide_opp_r.
-      apply div_unsigned_repr.
-      apply align_size_chunk_divides.
-      apply align_Mptr_modulus.
-      apply align_Mptr_modulus.
-      apply align_Mptr_modulus.
-    Qed.
-
-    Lemma align_Mptr_add:
-      forall o,
-        (align_chunk Mptr | Ptrofs.unsigned o) ->
-        (align_chunk Mptr | Ptrofs.unsigned (Ptrofs.add o (Ptrofs.repr (size_chunk Mptr)))).
-    Proof.
-      intros.
-      apply div_ptr_add; auto.
-      apply div_unsigned_repr.
-      apply align_size_chunk_divides.
-      apply align_Mptr_modulus.
-      apply align_Mptr_modulus.
-    Qed.
-
-    Lemma align_Mptr_add_gen:
-      forall o d,
-        (align_chunk Mptr | Ptrofs.unsigned o) ->
-        (align_chunk Mptr | Ptrofs.unsigned d) ->
-        (align_chunk Mptr | Ptrofs.unsigned (Ptrofs.add o d)).
-    Proof.
-      intros.
-      apply div_ptr_add; auto.
-      apply align_Mptr_modulus.
-    Qed.
-
-    Definition asm_prog_no_rsp (ge: Genv.t Asm.fundef unit):=
-      forall b f,
-        Genv.find_funct_ptr ge b = Some (Internal f) ->
-        asm_code_no_rsp (fn_code f).
-
-    Definition wf_asm_prog (ge: Genv.t Asm.fundef unit):=
-      forall b f,
-        Genv.find_funct_ptr ge b = Some (Internal f) ->
-        wf_asm_function f.
-
-    Lemma real_asm_inv_inv:
-      forall (prog_no_rsp: asm_prog_no_rsp ge) (WF: wf_asm_prog ge) s1 t s2,
-        step ge s1 t s2 ->
-        real_asm_inv s1 ->
-        real_asm_inv s2.
-    Proof.
-      intros prog_no_rsp WF s1 t s2 STEP INV; inv STEP.
-      - destruct (stk_unrelated_instr i) eqn:INVAR.
-        eapply exec_instr_invar_inv; eauto.
-        eapply prog_no_rsp; eauto. eapply Asmgenproof0.find_instr_in; eauto.
-        destruct i; simpl in INVAR; try congruence.
-        + (* call_s *)
-          simpl in H2. destr_in H2. inv H2. inv INV; constructor; simpl.
-          * red. simpl. simpl_regs. destruct RSPPTR as (o & EQ & AL); simpl in *; rewrite EQ.
-            simpl. eexists; split; eauto. apply align_Mptr_sub; auto.
-          * red in BSTACKPERM; red; simpl in *.
-            intros o k p. erewrite storev_perm; eauto. intro. erewrite storev_perm; eauto.
-          * red in STOP; red; simpl in *. erewrite <- Mem.support_storev; eauto.
-        + (* call_r *)
-          simpl in H2. destr_in H2. inv H2. inv INV; constructor; simpl.
-          * red. simpl. simpl_regs. destruct RSPPTR as (o & EQ & AL); simpl in *; rewrite EQ.
-            simpl. eexists; split; eauto. apply align_Mptr_sub; auto.
-          * red in BSTACKPERM; red; simpl in *.
-            intros o k p. erewrite storev_perm; eauto. intro. erewrite storev_perm; eauto.
-          * red in STOP; red; simpl in *. erewrite <- Mem.support_storev; eauto.
-        + (* ret *)
-          simpl in H2; repeat destr_in H2; inv INV; constructor; simpl.
-          * red. simpl. simpl_regs. destruct RSPPTR as (o & EQ & AL); simpl in *; rewrite EQ.
-            simpl. eexists; split; eauto. apply align_Mptr_add; auto.
-          * red in BSTACKPERM; red; simpl in *.
-            intros o k p. eauto.
-          * red in STOP; red; simpl in *. eauto.
-        + (* allocframe *)
-          simpl in H2; repeat destr_in H2; inv INV; constructor; simpl.
-          * red. simpl. simpl_regs. destruct RSPPTR as (o & EQ & AL); simpl in *; rewrite EQ.
-            simpl. eexists; split; eauto. apply align_Mptr_add_gen; auto.
-            unfold Ptrofs.neg. apply div_unsigned_repr; auto. apply Z.divide_opp_r.
-            unfold Ptrofs.sub. apply div_unsigned_repr; auto.
-            apply Z.divide_sub_r.
-            apply div_unsigned_repr; auto.
-            transitivity 8. unfold Mptr. destr; simpl. exists 1; lia. exists 2; lia. apply align_divides. lia.
-            apply align_Mptr_modulus.
-            apply div_unsigned_repr; auto.
-            apply align_size_chunk_divides.
-            apply align_Mptr_modulus.
-            apply align_Mptr_modulus.
-            apply align_Mptr_modulus.
-          * red in BSTACKPERM; red; simpl in *.
-            intros o k p. erewrite storev_perm; eauto. intro. erewrite storev_perm; eauto.
-          * red in STOP; red; simpl in *. erewrite <- Mem.support_storev; eauto.
-        + (* freeframe *)
-          simpl in H2; repeat destr_in H2; inv INV; constructor; simpl.
-          * red. simpl. simpl_regs. destruct RSPPTR as (o & EQ & AL); simpl in *; rewrite EQ.
-            simpl. eexists; split; eauto. apply align_Mptr_add_gen; auto.
-            unfold Ptrofs.sub. apply div_unsigned_repr; auto.
-            apply Z.divide_sub_r.
-            apply div_unsigned_repr; auto.
-            transitivity 8. unfold Mptr. destr; simpl. exists 1; lia. exists 2; lia. apply align_divides. lia.
-            apply align_Mptr_modulus.
-            apply div_unsigned_repr; auto.
-            apply align_size_chunk_divides.
-            apply align_Mptr_modulus.
-            apply align_Mptr_modulus.
-          * red in BSTACKPERM; red; eauto.
-          * red in STOP; red; eauto.
-      - inv INV; constructor.
-        + red in RSPPTR; red; simpl in *. unfold nextinstr_nf. repeat simpl_regs.
-          rewrite Asmgenproof0.undef_regs_other.
-          2: simpl; intuition subst; congruence.
-          exploit wf_asm_builtin_not_PC; eauto.
-          intros (NPC & NRSP & NRA).
-          rewrite set_res_other; auto.
-          rewrite Asmgenproof0.undef_regs_other.
-          eauto. setoid_rewrite in_map_iff. intros r' (x & PREG & IN). subst.
-          intro EQ. symmetry in EQ. apply preg_of_not_rsp in EQ. congruence.
-        + red in BSTACKPERM; red. simpl in *. intros o k p.
-          repeat erewrite (external_perm_stack _ _ _ _ _ _ _ _ _ _ _ H3); eauto.
-           simpl. auto. red in STOP; simpl in STOP. unfold bstack. unfold stkblock.
-           simpl. destruct STOP as (tl & st & STOP). rewrite STOP. split. auto. left. auto.
-           simpl. auto. red in STOP; simpl in STOP. unfold bstack. unfold stkblock.
-           simpl. destruct STOP as (tl & st & STOP). rewrite STOP. split. auto. left. auto.
-        + red in STOP; red; simpl in *. destruct STOP as (tl & st & STOP).
-          exploit external_call_stack; eauto. destr. intros.
-          rewrite STOP in H4. simpl in H4. destruct st. eauto. eauto.
-          intros. rewrite H4. eauto.
-      - inv INV; constructor.
-        + Opaque destroyed_at_call.
-          red in RSPPTR; red; simpl in *. repeat simpl_regs.
-          destruct RSPPTR as (o & EQ & AL); simpl in *. rewrite EQ.
-          simpl. eexists; split; eauto. apply align_Mptr_add; auto.
-        + red in BSTACKPERM; red. simpl in *. intros o k p.
-          repeat erewrite (external_perm_stack _ _ _ _ _ _ _ _ _ _ _ H2); eauto.
-           simpl. auto. red in STOP; simpl in STOP. unfold bstack. unfold stkblock.
-           simpl. destruct STOP as (tl & st & STOP). rewrite STOP. split. auto. left. auto.
-           simpl. auto. red in STOP; simpl in STOP. unfold bstack. unfold stkblock.
-           simpl. destruct STOP as (tl & st & STOP). rewrite STOP. split. auto. left. auto.
-        + red in STOP; red; simpl in *. destruct STOP as (tl & st & STOP).
-          exploit external_call_stack; eauto. destr. intros.
-          rewrite STOP in H3. simpl in H3. destruct st. eauto. eauto.
-          intros. rewrite H3. eauto.
-    Qed.
-
-End INVARIANT.
-
 
 Section WITHGETGE.
 
@@ -1726,7 +702,7 @@ Section WITHGETGE.
 
     Lemma exec_valid_instr_same : forall (i:instruction) f f' i rs m,
         instr_valid i ->
-        exec_instr ge f i rs m = exec_instr tge f' i rs m.
+        exec_instr ge f i rs m = exec_instr  tge f' i rs m.
     Proof.
       intros i f f' i0 rs m VI.
       destruct i0; cbn; auto;
@@ -1750,6 +726,13 @@ Section WITHGETGE.
       - erewrite SADDR_EQ. auto.
     Qed.
 
+(*    Lemma label_pos_1_eq: forall lbl z c,
+      Asm.label_pos lbl z c = label_pos instr_size_1 lbl z c.
+    Proof.
+      intros.
+      unfold instr_size_1. simpl. reflexivity.
+    Qed. *)
+
     Lemma goto_label_eq : forall (i:instruction) f f' l rs m,
         (forall lbl ofs, label_pos lbl ofs (fn_code f) = label_pos lbl ofs (fn_code f')) ->
         goto_label ge f l rs m = goto_label tge f' l rs m.
@@ -1762,7 +745,7 @@ Section WITHGETGE.
         exploit fptr_some_eq; eauto.
         intros (f1 & FT). rewrite FT. auto.
         rewrite FPTR_EQ in Heqo0. rewrite Heqo0. auto.
-      - rewrite <- H. rewrite Heqo. auto.
+      - rewrite <- H. setoid_rewrite Heqo. auto.
     Qed.
 
     Lemma exec_instr_same : forall (i:instruction) f f' i rs m,
@@ -1838,3 +821,968 @@ Section RECEPTIVEDET.
   Qed.
 
 End RECEPTIVEDET.
+
+Section WFASM.
+
+  Fixpoint in_builtin_arg (b: builtin_arg preg) (r: preg) :=
+    match b with
+    | BA x => if preg_eq r x then True else False
+    | BA_splitlong ba1 ba2 => in_builtin_arg ba1 r \/ in_builtin_arg ba2 r
+    | BA_addptr ba1 ba2 => in_builtin_arg ba1 r \/ in_builtin_arg ba2 r
+    | _ => False
+    end.
+
+  Inductive is_alloc : instruction -> Prop :=
+    is_alloc_intro sz ora olink:
+      is_alloc (Pallocframe sz ora olink).
+
+  Definition make_palloc f  : instruction :=
+    let sz := fn_stacksize f in
+    (Pallocframe sz (Ptrofs.sub (Ptrofs.repr (align sz 8)) (Ptrofs.repr (size_chunk Mptr))) (fn_ofs_link f)).
+
+  Lemma make_palloc_is_alloc:
+    forall f,
+      is_alloc (make_palloc f).
+  Proof. constructor. Qed.
+
+  Inductive is_free : instruction -> Prop :=
+    is_free_intro sz ora olink:
+      is_free (Pfreeframe sz ora olink).
+
+  Lemma is_free_dec:
+    forall i,
+      {is_free i} + {~ is_free i}.
+  Proof.
+    destruct i; try now (right; intro A; inv A).
+    left. econstructor; eauto.
+  Defined.
+  Inductive is_jmp: instruction -> Prop :=
+  | is_jmps_intro: forall i sg, is_jmp (Pjmp_s i sg)
+  | is_jmpr_intro: forall ir sg, is_jmp (Pjmp_r ir sg).
+
+
+  Inductive intermediate_instruction : instruction -> Prop :=
+  | ii_alloc i: is_alloc i -> intermediate_instruction i
+  | ii_jmp i: i = Pret \/ is_jmp i -> intermediate_instruction i.
+
+  Record wf_asm_function (f: function): Prop :=
+    {
+
+      wf_asm_alloc_only_at_beginning:
+        forall o sz ora olink,
+          find_instr o (fn_code f) = Some (Pallocframe sz ora olink) ->
+          o = 0;
+
+      wf_asm_alloc_at_beginning:
+        find_instr 0 (fn_code f) = Some (make_palloc f);
+
+      wf_asm_after_freeframe:
+        forall i o,
+          find_instr (Ptrofs.unsigned o) (fn_code f) = Some i ->
+          is_free i ->
+          exists i' ,
+            find_instr (Ptrofs.unsigned (Ptrofs.add o (Ptrofs.repr (instr_size i)))) (fn_code f) = Some i' /\
+            (i' = Pret \/ is_jmp i' );
+
+      wf_asm_ret_jmp_comes_after_freeframe:
+        forall i o,
+          find_instr (Ptrofs.unsigned o) (fn_code f) = Some i ->
+          i = Pret \/ is_jmp i ->
+          exists o' ifree,
+            find_instr (Ptrofs.unsigned o') (fn_code f) = Some ifree /\
+            is_free ifree /\
+            Ptrofs.unsigned o' + instr_size ifree = Ptrofs.unsigned o;
+
+      wf_asm_code_bounded:
+        0 <= code_size (fn_code f) <= Ptrofs.max_unsigned;
+
+      wf_asm_builtin_not_PC:
+        forall o ef args res,
+          find_instr o (fn_code f) = Some (Pbuiltin ef args res) ->
+          ~ in_builtin_res res PC /\
+          ~ in_builtin_res res RSP
+          /\ Forall (fun arg : builtin_arg preg => ~ in_builtin_arg arg RA) args;
+
+      wf_asm_jmp_no_rsp:
+        forall o (r: ireg) sg,
+          find_instr o (fn_code f) = Some (Pjmp_r r sg) ->
+          r <> RSP;
+
+      wf_asm_call_no_rsp:
+        forall o (r: ireg) sg,
+          find_instr o (fn_code f) = Some (Pcall_r r sg) ->
+          r <> RSP;
+
+      wf_asm_free_spec:
+        forall o sz ora olink,
+          find_instr o (fn_code f) = Some (Pfreeframe sz ora olink) ->
+          sz = fn_stacksize f /\ ora = Ptrofs.sub (Ptrofs.repr (align sz 8)) (Ptrofs.repr (size_chunk Mptr));
+
+      wf_allocframe_repr:
+        forall o sz ora olink,
+          find_instr o (fn_code f) = Some (Pallocframe sz ora olink) ->
+          align sz 8 - size_chunk Mptr =
+          Ptrofs.unsigned (Ptrofs.sub (Ptrofs.repr (align sz 8)) (Ptrofs.repr (size_chunk Mptr)));
+
+      wf_freeframe_repr:
+        forall o sz ora olink,
+          find_instr o (fn_code f) = Some (Pfreeframe sz ora olink) ->
+          Ptrofs.repr (align sz 8 - size_chunk Mptr) = Ptrofs.sub (Ptrofs.repr (align sz 8)) (Ptrofs.repr (size_chunk Mptr));
+    }.
+
+  Definition is_make_palloc a f :=  a = make_palloc f /\
+                                    align (fn_stacksize f) 8 - size_chunk Mptr =
+                                    Ptrofs.unsigned (Ptrofs.sub (Ptrofs.repr (align (fn_stacksize f) 8)) (Ptrofs.repr (size_chunk Mptr))).
+(*
+  Lemma pair_eq: forall {A B}
+                   (Adec: forall (a b: A), {a = b} + {a <> b})
+                   (Bdec: forall (a b: B), {a = b} + {a <> b}),
+      forall (a b: A * B), {a = b} + {a <> b}.
+  Proof.
+    intros.
+    destruct a, b.
+    destruct (Adec a a0), (Bdec b b0); subst;
+      first [ now (right; inversion 1; congruence)
+            | left; reflexivity ].
+  Defined.
+*)
+  Definition pallocframe_dec s s' o o' l l':
+    {Pallocframe s o l= Pallocframe s' o' l'} + {Pallocframe s o l <> Pallocframe s' o' l'}.
+  Proof.
+    destruct (zeq s s'); subst. 2: (now right; inversion 1).
+    destruct (Ptrofs.eq_dec o o'); subst. 2: (now right; inversion 1).
+    destruct (Ptrofs.eq_dec l l'); subst. 2: (now right; inversion 1).
+    left; reflexivity.
+  Defined.
+
+  Lemma and_dec: forall {A B: Prop},
+      { A } + { ~ A } ->
+      { B } + { ~ B } ->
+      { A /\ B } + { ~ (A /\ B) }.
+  Proof.
+    intros. destruct H, H0; [left|right|right|right]; intuition.
+  Qed.
+
+  Definition is_make_palloc_dec a f : { is_make_palloc a f } + { ~ is_make_palloc a f }.
+  Proof.
+    unfold is_make_palloc, make_palloc.
+    destruct a; try (now right; inversion 1).
+    apply and_dec.
+    apply pallocframe_dec.
+    apply zeq.
+  Defined.
+
+  Definition check_ret_or_jmp roj :=
+    match roj with
+    | Pret |Pjmp_r _ _ | Pjmp_s _ _=> true
+    | _ => false
+    end.
+
+  Definition valid_ret_or_jmp roj :=
+    match roj with
+    | Pjmp_r r _ =>  negb (preg_eq r RSP)
+    | _ => true
+    end.
+
+  Definition check_free f sz ora :=
+      sz = fn_stacksize f /\ ora = Ptrofs.sub (Ptrofs.repr (align sz 8)) (Ptrofs.repr (size_chunk Mptr)) /\
+      Ptrofs.repr (align sz 8 - size_chunk Mptr) = Ptrofs.sub (Ptrofs.repr (align sz 8)) (Ptrofs.repr (size_chunk Mptr)).
+
+  Definition check_free_dec f sz ora : { check_free f sz ora } + { ~ check_free f sz ora }.
+  Proof.
+    unfold check_free.
+    apply and_dec. 2: apply and_dec.
+    apply zeq. apply Ptrofs.eq_dec. apply Ptrofs.eq_dec.
+  Defined.
+
+  Definition check_builtin args res :=
+    ~ in_builtin_res res PC /\
+    ~ in_builtin_res res RSP
+    /\ Forall (fun arg : builtin_arg preg => ~ in_builtin_arg arg RA) args.
+
+  Lemma not_in_builtin_res_dec res r:
+    {~ in_builtin_res res r} + {~ ~ in_builtin_res res r}.
+  Proof.
+    induction res; simpl.
+    destruct (preg_eq x r); subst; intuition. left; inversion 1.
+    destruct IHres1, IHres2; try (right; now intuition). left. intuition congruence.
+  Qed.
+
+
+  Lemma not_in_builtin_arg_dec arg r:
+    {~ in_builtin_arg arg r} + {~ ~ in_builtin_arg arg r}.
+  Proof.
+    induction arg; simpl; try (try destr; left; now inversion 1).
+    destruct IHarg1, IHarg2; try (right; now intuition). left. intuition congruence.
+    destruct IHarg1, IHarg2; try (right; now intuition). left. intuition congruence.
+  Qed.
+
+  Definition check_builtin_dec args res: {check_builtin args res} + { ~ check_builtin args res}.
+  Proof.
+    unfold check_builtin.
+    repeat apply and_dec.
+    apply not_in_builtin_res_dec.
+    apply not_in_builtin_res_dec.
+    apply Forall_dec. intros.
+    apply not_in_builtin_arg_dec.
+  Defined.
+
+  Hypothesis instr_size_repr : forall i, 0 <= instr_size i <= Ptrofs.max_unsigned.
+  Hypothesis instr_size_positive : forall i, 0 < instr_size i.
+
+  Lemma code_size_non_neg: forall c, 0 <= code_size c.
+  Proof.
+    intros. induction c; simpl. lia. generalize (instr_size_positive a); lia.
+  Qed.
+
+  Lemma find_instr_bound:
+    forall c o i,
+      find_instr o c = Some i ->
+      o + instr_size i <= code_size c.
+  Proof.
+    induction c; simpl; intros; eauto. congruence.
+    destr_in H. inv H. generalize (code_size_non_neg c) (instr_size_positive i). lia.
+    apply IHc in H. lia.
+  Qed.
+
+  Lemma find_instr_pos_positive:
+        forall c o i,
+          find_instr o c = Some i ->
+          0 <= o.
+   Proof.
+     induction c; intros; simpl; inv H. destr_in H1. lia.
+     eapply IHc in H1. generalize (instr_size_positive a). lia.
+   Qed.
+(*
+  Lemma instr_size_repr : 0 <= 1 <= Ptrofs.max_unsigned.
+  Proof.
+    vm_compute. split; congruence.
+  Qed.*)
+
+  Lemma code_bounded_repr':
+    forall c
+      (RNG: 0 <= code_size c <= Ptrofs.max_unsigned)
+      i o
+      (FI: find_instr o c = Some i)
+      sz
+      (LE: 0 <= sz <= instr_size i),
+      Ptrofs.unsigned (Ptrofs.add (Ptrofs.repr o) (Ptrofs.repr sz)) = o + sz.
+  Proof.
+    intros.
+    unfold Ptrofs.add.
+    rewrite (Ptrofs.unsigned_repr sz). 2: generalize (instr_size_repr i); lia.
+    generalize (find_instr_bound _ _ _ FI) (find_instr_pos_positive _ _ _ FI). intros.
+    rewrite (Ptrofs.unsigned_repr o) by lia.
+    apply Ptrofs.unsigned_repr; lia.
+  Qed.
+
+  Lemma code_bounded_repr:
+    forall c
+      (RNG: 0 <= code_size c <= Ptrofs.max_unsigned)
+      i o
+      (FI: find_instr (Ptrofs.unsigned o) c = Some i)
+      sz
+      (LE: 0 <= sz <= instr_size i),
+      Ptrofs.unsigned (Ptrofs.add o (Ptrofs.repr sz)) = Ptrofs.unsigned o + sz.
+  Proof.
+    intros.
+    erewrite <- code_bounded_repr'; eauto.
+    unfold Ptrofs.add.
+    rewrite Ptrofs.repr_unsigned. reflexivity.
+  Qed.
+
+  Lemma wf_asm_pc_repr' : forall f : function,
+       wf_asm_function f ->
+       forall (i : instruction) (o : ptrofs),
+       find_instr (Ptrofs.unsigned o) (fn_code f) = Some i ->
+       forall sz : Z, 0 <= sz <= instr_size i ->
+       Ptrofs.unsigned (Ptrofs.add o (Ptrofs.repr sz)) = Ptrofs.unsigned o + sz.
+  Proof.
+    intros; eapply code_bounded_repr; eauto.
+    apply wf_asm_code_bounded; eauto.
+  Qed.
+
+  Fixpoint check_asm_body (f: function) (next_roj: bool) (r: code) : bool :=
+    match r with
+    | nil => negb next_roj
+    | i :: r =>
+      let roj := proj_sumbool (is_free_dec i) in
+      check_asm_body f roj r &&
+      if next_roj then check_ret_or_jmp i && valid_ret_or_jmp i
+      else
+        negb (check_ret_or_jmp i) &&
+        match i with
+        | Pfreeframe sz ora olink =>     (* after a free, ret or jmp *)
+          check_free_dec f sz ora
+        | Pallocframe _ _ _ => false (* no alloc in body *)
+        | Pcall_r r sg => negb (preg_eq r RSP)
+        | Pbuiltin _ args res => check_builtin_dec args res
+        | _ => true
+      end
+    end.
+
+  Definition wf_asm_function_check (f: function) : bool :=
+    match fn_code f with
+    | nil => false
+    | a::r => is_make_palloc_dec a f && check_asm_body f false r
+    end && zle (code_size (fn_code f)) Ptrofs.max_unsigned.
+
+  Lemma check_asm_body_no_alloc:
+    forall f c b i,
+      check_asm_body f b c = true ->
+      In i c ->
+      ~ is_alloc i.
+  Proof.
+    induction c; simpl; intros. easy.
+    intro IA. inv IA.
+    assert (exists b, check_asm_body f b c = true).
+    {
+      eexists. refine (proj1 _); apply andb_true_iff; eauto.
+    }
+    destruct H1.
+    destruct H0. subst. simpl in *.
+    apply andb_true_iff in H. destruct H. destr_in H0.
+    eapply IHc in H0; eauto. apply H0; constructor.
+  Qed.
+
+  Lemma find_instr_app:
+    forall a o b,
+      0 <= o ->
+      find_instr (o + code_size a) (a ++ b) = find_instr o b.
+  Proof.
+    induction a; simpl; intros; eauto.
+    f_equal. lia.
+    rewrite pred_dec_false.
+    rewrite <- (IHa o b). f_equal. lia. lia.
+    generalize (code_size_non_neg a0). generalize (instr_size_positive a). lia.
+  Qed.
+
+  Lemma find_instr_app':
+    forall a o b,
+      code_size a <= o ->
+      find_instr o (a ++ b) = find_instr (o - code_size a) b.
+  Proof.
+    intros.
+    rewrite <- (find_instr_app a _ b). f_equal. lia. lia.
+  Qed.
+
+  Lemma find_instr_split:
+    forall c o i,
+      find_instr o c = Some i ->
+      exists a b, c = a ++ i :: b /\ o = code_size a.
+  Proof.
+    induction c; simpl; intros; eauto. congruence.
+    destr_in H. inv H. eexists nil, c; simpl. split; auto.
+    edestruct IHc as (aa & b & EQ & SZ). apply H. subst.
+    exists (a::aa), b; simpl; split; auto.
+    generalize (instr_size_positive a). lia.
+  Qed.
+
+  Lemma find_instr_app_pres: forall f1 f2 ofs i,
+      find_instr ofs f1 = Some i ->
+      find_instr ofs (f1 ++ f2) = Some i.
+  Proof.
+    induction f1 as [|i1 f1].
+    - cbn. intros; congruence.
+    - cbn. intros f2 i FI.
+      destr. eauto.
+  Qed.
+
+  Lemma code_size_app:
+    forall c1 c2,
+      code_size (c1 ++ c2) = code_size c1 + code_size c2.
+  Proof.
+    induction c1; simpl; intros; eauto. rewrite IHc1. lia.
+  Qed.
+
+  Lemma check_asm_body_after_free:
+    forall f a i b roj,
+      check_asm_body f roj (a ++ i :: b) = true ->
+      is_free i ->
+      check_asm_body f true b = true.
+  Proof.
+    induction a; simpl; intros; eauto.
+    apply andb_true_iff in H. destruct H as (H & _).
+    inv H0. simpl in *. auto.
+    apply andb_true_iff in H. destruct H as (H & B).
+    destruct (is_free_dec a); simpl in *. inv i0.
+    eapply IHa; eauto.
+    eapply IHa; eauto.
+  Qed.
+
+
+  Lemma check_asm_body_call:
+    forall f c b r sg,
+      check_asm_body f b c = true ->
+      In (Pcall_r r sg) c ->
+      r <> RSP.
+  Proof.
+    induction c; simpl; intros. easy.
+    assert (exists b, check_asm_body f b c = true).
+    {
+      eexists. refine (proj1 _); apply andb_true_iff; eauto.
+    }
+    apply andb_true_iff in H. destruct H. destruct H1. destruct H0; eauto. subst. simpl in *.
+    destr_in H2; simpl in *.
+    unfold proj_sumbool in H2; destr_in H2. simpl in H2. congruence.
+  Qed.
+
+  Lemma check_asm_body_free:
+    forall f c b sz ora olink,
+      check_asm_body f b c = true ->
+      In (Pfreeframe sz ora olink) c ->
+      check_free f sz ora.
+  Proof.
+    induction c; simpl; intros. easy.
+    assert (exists b, check_asm_body f b c = true).
+    {
+      eexists. refine (proj1 _); apply andb_true_iff; eauto.
+    }
+    apply andb_true_iff in H. destruct H. destruct H1. destruct H0; eauto. subst. simpl in *.
+    destr_in H2; simpl in *.
+    unfold proj_sumbool in H2; destr_in H2.
+  Qed.
+
+  Lemma check_asm_body_before_roj:
+    forall f a i b roj,
+      check_asm_body f roj (a ++ i :: b) = true ->
+      i = Pret \/ is_jmp i ->
+      (a = nil /\ roj = true) \/ exists a0 i0, a = a0 ++ i0 :: nil /\ is_free i0.
+  Proof.
+    induction a; simpl; intros; eauto.
+    - apply andb_true_iff in H. destruct H as (A & B).
+      destruct H0 as [ROJ|ROJ]; inv ROJ; simpl in *. destr_in B.
+      destruct roj. auto. congruence. destr_in B.
+    - apply andb_true_iff in H. destruct H as (A & B).
+      destruct (is_free_dec a); simpl in *. inv i0.
+      + simpl in *. destr_in B. right.
+        destruct a0. clear IHa. simpl in *.
+        eexists nil, _. split. simpl. eauto. constructor.
+        edestruct IHa as [ROJ|(a1 & i1 & EQ & IFR)]; eauto.
+        destruct ROJ; congruence. rewrite EQ.
+        eexists (_ :: a1), i1; split. simpl. reflexivity. auto.
+      + edestruct IHa as [ROJ|(a1 & i1 & EQ & IFR)]; eauto.
+        destruct ROJ; congruence. subst. right.
+        eexists (_ :: a1), i1; split. simpl. reflexivity. auto.
+  Qed.
+
+  Lemma check_asm_body_builtin:
+    forall f c b ef args res,
+      check_asm_body f b c = true ->
+      In (Pbuiltin ef args res) c ->
+      check_builtin args res.
+  Proof.
+    induction c; simpl; intros. easy.
+    assert (exists b, check_asm_body f b c = true).
+    {
+      eexists. refine (proj1 _); apply andb_true_iff; eauto.
+    }
+    destruct H1.
+    destruct H0. subst. simpl in *.
+    apply andb_true_iff in H. destruct H. destr_in H0.
+    unfold proj_sumbool in H0; destr_in H0.
+    eapply IHc in H0; eauto.
+  Qed.
+
+  Lemma check_asm_body_jmp:
+    forall f c b r sg,
+      check_asm_body f b c = true ->
+      In (Pjmp_r  r sg) c ->
+      r <> RSP.
+  Proof.
+    induction c; simpl; intros. easy.
+    assert (exists b, check_asm_body f b c = true).
+    {
+      eexists. refine (proj1 _); apply andb_true_iff; eauto.
+    }
+    apply andb_true_iff in H. destruct H. destruct H1. destruct H0; eauto. subst. simpl in *.
+    destr_in H2; simpl in *.
+    unfold proj_sumbool in H2; destr_in H2. simpl in H2. congruence.
+  Qed.
+
+  Lemma find_instr_in:
+    forall c pos i,
+      find_instr pos c = Some i -> In i c.
+  Proof.
+    induction c; simpl. intros; discriminate.
+    intros until i. case (zeq pos 0); intros.
+    left; congruence. right; eauto.
+  Qed.
+
+  Lemma wf_asm_function_check_correct f:
+    wf_asm_function_check f = true ->
+    wf_asm_function f.
+  Proof.
+    unfold wf_asm_function_check. destr. simpl. congruence.
+    rewrite ! andb_true_iff. intros ((A & B) & C).
+    unfold proj_sumbool in A, C. destr_in A; destr_in C.
+    clear A C. rename Heqc into CODE. rename l into SIZE.
+    constructor.
+    - rewrite CODE. simpl. intros. destr_in H.
+      apply find_instr_in in H.
+      eapply check_asm_body_no_alloc in H; eauto. contradict H. constructor.
+    - rewrite CODE; simpl. clear - i0. destruct i0 as (A & B). subst. reflexivity.
+    - destruct i0 as (i0 & _). subst. rewrite CODE. simpl.
+      intros. destr_in H. inv H. inv H0.
+      simpl in SIZE.
+      rewrite pred_dec_false.
+      replace (Ptrofs.unsigned (Ptrofs.add o (Ptrofs.repr (instr_size i))) - instr_size (make_palloc f))
+        with (Ptrofs.unsigned (Ptrofs.add (Ptrofs.repr (Ptrofs.unsigned o - instr_size (make_palloc f))) (Ptrofs.repr (instr_size i)))).
+      revert H.
+      generalize (Ptrofs.unsigned o - instr_size (make_palloc f)).
+      intros. 
+      edestruct find_instr_split as (a & b & EQ & SZ). apply H. subst.
+      rewrite find_instr_app'.
+      simpl. rewrite pred_dec_false.
+      eapply check_asm_body_after_free in B; eauto.
+      destruct b; simpl in B. congruence. simpl. rewrite pred_dec_true. eexists; split; eauto.
+      apply andb_true_iff in B. destruct B as (B & CHK).
+      unfold check_ret_or_jmp in CHK. apply andb_true_iff in CHK. destruct CHK as (CHK & _). destr_in CHK; try (right; constructor).
+      unfold Ptrofs.add.
+      rewrite (Ptrofs.unsigned_repr (code_size a)).
+      rewrite (Ptrofs.unsigned_repr _ (instr_size_repr i)).
+      rewrite Ptrofs.unsigned_repr. lia.
+      simpl in SIZE. rewrite code_size_app in SIZE. simpl in SIZE.
+      generalize (code_size_non_neg a) (instr_size_positive i) (instr_size_positive i0) (code_size_non_neg b)
+                 (instr_size_positive (make_palloc f)). lia.
+      simpl in SIZE. rewrite code_size_app in SIZE. simpl in SIZE.
+      generalize (code_size_non_neg a) (instr_size_positive i) (instr_size_positive i0) (code_size_non_neg b)
+                 (instr_size_positive (make_palloc f)). lia.
+      unfold Ptrofs.add.
+      rewrite (Ptrofs.unsigned_repr (code_size a)).
+      rewrite (Ptrofs.unsigned_repr _ (instr_size_repr i)).
+      rewrite Ptrofs.unsigned_repr. generalize (instr_size_positive i); lia.
+      simpl in SIZE. rewrite code_size_app in SIZE. simpl in SIZE.
+      generalize (code_size_non_neg a) (instr_size_positive i) (code_size_non_neg b)
+                 (instr_size_positive (make_palloc f)). lia.
+      simpl in SIZE. rewrite code_size_app in SIZE. simpl in SIZE.
+      generalize (code_size_non_neg a) (instr_size_positive i) (code_size_non_neg b)
+                 (instr_size_positive (make_palloc f)). lia.
+      unfold Ptrofs.add.
+      rewrite (Ptrofs.unsigned_repr (code_size a)).
+      rewrite (Ptrofs.unsigned_repr _ (instr_size_repr i)).
+      rewrite Ptrofs.unsigned_repr. generalize (instr_size_positive i); lia.
+      simpl in SIZE. rewrite code_size_app in SIZE. simpl in SIZE.
+      generalize (code_size_non_neg a) (instr_size_positive i) (code_size_non_neg b)
+                 (instr_size_positive (make_palloc f)). lia.
+      simpl in SIZE. rewrite code_size_app in SIZE. simpl in SIZE.
+      generalize (code_size_non_neg a) (instr_size_positive i) (code_size_non_neg b)
+                 (instr_size_positive (make_palloc f)). lia.
+      unfold Ptrofs.add.
+      rewrite (Ptrofs.unsigned_repr _ (instr_size_repr i)).
+      rewrite (Ptrofs.unsigned_repr (Ptrofs.unsigned o - _)).
+      rewrite ! Ptrofs.unsigned_repr. lia.
+      generalize (find_instr_bound _ _ _ H) (find_instr_pos_positive _ _ _ H).
+      generalize (instr_size_positive i)
+                 (instr_size_positive (make_palloc f)). lia.
+      generalize (find_instr_bound _ _ _ H) (find_instr_pos_positive _ _ _ H).
+      generalize (instr_size_positive i)
+                 (instr_size_positive (make_palloc f)). lia.
+      generalize (find_instr_bound _ _ _ H) (find_instr_pos_positive _ _ _ H).
+      generalize (instr_size_positive i)
+                 (instr_size_positive (make_palloc f)). lia.
+      unfold Ptrofs.add.
+      rewrite (Ptrofs.unsigned_repr _ (instr_size_repr i)).
+      rewrite Ptrofs.unsigned_repr.
+      generalize (Ptrofs.unsigned_range o) (instr_size_positive i); lia.
+      generalize (find_instr_bound _ _ _ H) (find_instr_pos_positive _ _ _ H).
+      generalize (instr_size_positive i)
+                 (instr_size_positive (make_palloc f)). lia.
+    - destruct i0 as (i0 & _). subst. rewrite CODE. simpl.
+      intros i o FI ROJ.
+      destr_in FI. inv FI. destruct ROJ as [ROJ|ROJ]; inv ROJ.
+      edestruct find_instr_split as (a & b & EQ & SZ). apply FI. subst.
+      destruct (check_asm_body_before_roj _ _ _ _ _ B ROJ) as [(NIL & ROJFALSE)|(a0 & i0 & EQ & IFR)]. congruence.
+      subst.
+      exists (Ptrofs.sub o (Ptrofs.repr (instr_size i0))), i0.
+      rewrite pred_dec_false.
+      replace (Ptrofs.unsigned (Ptrofs.sub o (Ptrofs.repr (instr_size i0))) - instr_size (make_palloc f)) 
+        with (0 + code_size a0). rewrite app_ass.
+      rewrite find_instr_app. simpl. split; auto. split. auto.
+      unfold Ptrofs.sub. 
+      rewrite (Ptrofs.unsigned_repr _ (instr_size_repr i0)).
+      rewrite Ptrofs.unsigned_repr. lia.
+      generalize (find_instr_bound _ _ _ FI) (find_instr_pos_positive _ _ _ FI). intros.
+      simpl in *. rewrite ! code_size_app in *. simpl in *.
+      generalize (code_size_non_neg a0) (instr_size_positive i) (instr_size_positive i0) (code_size_non_neg b)
+                 (instr_size_positive (make_palloc f)). lia.
+      lia.
+      unfold Ptrofs.sub. 
+      rewrite (Ptrofs.unsigned_repr _ (instr_size_repr i0)).
+      rewrite Ptrofs.unsigned_repr.
+      simpl in *. rewrite ! code_size_app in *. simpl in *. lia.
+      generalize (find_instr_bound _ _ _ FI) (find_instr_pos_positive _ _ _ FI). intros.
+      simpl in *. rewrite ! code_size_app in *. simpl in *.
+      generalize (code_size_non_neg a0) (instr_size_positive i) (instr_size_positive i0) (code_size_non_neg b)
+                 (instr_size_positive (make_palloc f)). lia.
+      unfold Ptrofs.sub. 
+      rewrite (Ptrofs.unsigned_repr _ (instr_size_repr i0)).
+      rewrite Ptrofs.unsigned_repr.
+      simpl in *. rewrite ! code_size_app in *. simpl in *.
+      generalize (find_instr_bound _ _ _ FI) (find_instr_pos_positive _ _ _ FI). intros. 
+      simpl in *. rewrite ! code_size_app in *. simpl in *.
+      generalize (code_size_non_neg a0) (instr_size_positive i) (instr_size_positive i0) (code_size_non_neg b)
+                 (instr_size_positive (make_palloc f)). lia.
+      generalize (find_instr_bound _ _ _ FI) (find_instr_pos_positive _ _ _ FI). intros. 
+      simpl in *. rewrite ! code_size_app in *. simpl in *.
+      generalize (code_size_non_neg a0) (instr_size_positive i) (instr_size_positive i0) (code_size_non_neg b)
+                 (instr_size_positive (make_palloc f)). lia.
+    - rewrite CODE; split; auto.
+      generalize (code_size_non_neg (i::c)). lia.
+    - destruct i0 as (i0 & _). subst. rewrite CODE. simpl.
+      intros o ef args res FI.
+      destr_in FI. inv FI.
+      apply find_instr_in in FI.
+      eapply check_asm_body_builtin in FI; eauto.
+    - destruct i0 as (i0 & _). subst. rewrite CODE. simpl.
+      intros o r sg FI.
+      destr_in FI. inv FI.
+      apply find_instr_in in FI.
+      eapply check_asm_body_jmp in FI; eauto.
+    - destruct i0 as (i0 & _). subst. rewrite CODE. simpl.
+      intros o r sg FI.
+      destr_in FI. inv FI.
+      apply find_instr_in in FI.
+      eapply check_asm_body_call in FI; eauto.
+    - destruct i0 as (i0 & _). subst. rewrite CODE. simpl.
+      intros o sz ora olink FI.
+      destr_in FI. inv FI.
+      apply find_instr_in in FI.
+      edestruct check_asm_body_free as (A & BB & C); subst; eauto.
+    - destruct i0 as (i0 & PA). subst. rewrite CODE. simpl.
+      intros o sz ora olink FI.
+      destr_in FI. inv FI; auto.
+      apply find_instr_in in FI.
+      eapply check_asm_body_no_alloc in FI; eauto. contradict FI; constructor.
+    - destruct i0 as (i0 & _). subst. rewrite CODE. simpl.
+      intros o sz ora olink FI.
+      destr_in FI. inv FI.
+      apply find_instr_in in FI.
+      edestruct check_asm_body_free as (A & BB & C); subst; eauto.
+  Qed.
+
+  Lemma wf_asm_pc_repr:
+    forall f (WF: wf_asm_function f) i o,
+      find_instr (Ptrofs.unsigned o) (fn_code f) = Some i ->
+      Ptrofs.unsigned (Ptrofs.add o (Ptrofs.repr (instr_size i))) = Ptrofs.unsigned o + instr_size i.
+  Proof.
+    intros; eapply wf_asm_pc_repr'; eauto. generalize (instr_size_positive i); lia.
+  Qed.
+
+  Lemma wf_asm_wf_allocframe:
+    forall f (WF: wf_asm_function f) o sz ora olink
+      (FI: find_instr o (fn_code f) = Some (Pallocframe sz ora olink)),
+      make_palloc f = Pallocframe sz ora olink.
+  Proof.
+    intros.
+    exploit wf_asm_alloc_only_at_beginning; eauto. intro; subst.
+    erewrite wf_asm_alloc_at_beginning in FI; eauto. inv FI; auto.
+  Qed.
+
+End WFASM.
+
+End INSTRSIZE.
+(* RealAsm senmantic version 1: instr_size == 1*)
+
+Definition instr_size_1 : instruction -> Z := fun i => 1.
+
+
+Definition rs_state s :=
+  let '(State rs _) := s in rs.
+Definition m_state s :=
+  let '(State _ m) := s in m.
+
+  Section INVARIANT.
+
+    Variable prog: Asm.program.
+    Let ge := Genv.globalenv prog.
+
+    Definition bstack := stkblock.
+
+    Definition rsp_ptr (s: state) : Prop :=
+      exists o, rs_state s RSP = Vptr bstack o /\ (align_chunk Mptr | Ptrofs.unsigned o).
+
+    Definition bstack_perm (s: state) : Prop :=
+      forall o k p,
+        Mem.perm (m_state s) bstack o k p ->
+        Mem.perm (m_state s) bstack o k Writable.
+
+    Definition stack_top_state (s: state) : Prop :=
+      exists tl st, Mem.stack(Mem.support (m_state s))= Node None (1%positive::nil) tl st.
+
+    Inductive real_asm_inv : state -> Prop :=
+    | real_asm_inv_intro:
+        forall s
+          (RSPPTR: rsp_ptr s)
+          (BSTACKPERM: bstack_perm s)
+          (STOP: stack_top_state s),
+          real_asm_inv s.
+
+    Lemma storev_perm :
+      forall m chunk addr v m', Mem.storev chunk m addr v = Some m' ->
+                           (forall b o k p, Mem.perm m' b o k p <-> Mem.perm m b o k p).
+      Proof.
+        intros. unfold Mem.storev in H. destr_in H. split.
+        eapply Mem.perm_store_2; eauto. eapply Mem.perm_store_1; eauto.
+      Qed.
+
+    Lemma real_initial_inv:
+      forall is,
+        initial_state prog is -> real_asm_inv is.
+    Proof.
+      intros. inv H.
+      apply Genv.init_mem_stack in H0 as STK.
+      constructor.
+      - red. simpl. unfold rs0; simpl_regs. eexists. split. reflexivity.
+        apply div_ptr_add.
+        apply div_unsigned_repr.
+        apply Z.divide_add_r. apply align_Mptr_stack_limit. apply align_Mptr_align8.
+        apply align_Mptr_modulus. unfold Ptrofs.neg. apply div_unsigned_repr.
+        apply Zdivide_opp_r.
+        apply div_unsigned_repr.
+        apply align_size_chunk_divides.
+        apply align_Mptr_modulus.
+        apply align_Mptr_modulus.
+        apply align_Mptr_modulus.
+      - exploit Mem.alloc_result; eauto. intro. subst.
+        unfold Mem.nextblock in H1. unfold Mem.fresh_block in H1.
+        rewrite STK in H1. destr_in H1. simpl in Heqp. inv Heqp.
+        red. unfold bstack. unfold stkblock. intros o k p.
+        repeat erewrite (storev_perm _ _ _ _ _ H2). eauto.
+        intro. exploit Mem.perm_alloc_3; eauto.
+        intro. exploit Mem.perm_alloc_2; eauto. simpl. intro. eapply Mem.perm_implies; eauto.
+        apply perm_F_any.
+      - red. simpl. apply Mem.stack_alloc in H1. rewrite STK in H1.
+        exists nil, None. simpl in H1. erewrite <- Mem.support_storev; eauto.
+Qed.
+
+(*    Lemma nextinstr_1_eq :
+      forall rs,
+        nextinstr rs Ptrofs.one = Asm.nextinstr rs.
+    Proof.
+      intros. reflexivity.
+    Qed. *)
+
+    Lemma exec_instr_invar_same:
+      forall f i rs1 m1,
+        stk_unrelated_instr i = true ->
+        exec_instr instr_size_1 ge f i rs1 m1 = SSAsm.exec_instr ge f i rs1 m1.
+    Proof.
+      intros f i rs1 m1 SI.
+      destruct i; simpl in SI; simpl; unfold instr_size_1; simpl; try reflexivity; congruence.
+    Qed.
+
+    Lemma exec_instr_invar_same':
+      forall f i rs1 m1,
+        stk_unrelated_instr i = true ->
+        Asm.exec_instr ge f i rs1 m1 = SSAsm.exec_instr ge f i rs1 m1.
+    Proof.
+      intros f i rs1 m1 SI.
+      destruct i; simpl in SI; simpl; try congruence.
+    Qed.
+
+    Lemma exec_instr_invar_inv:
+      forall f i rs1 m1 rs2 m2,
+        asm_instr_unchange_rsp i ->
+        stk_unrelated_instr i = true ->
+        exec_instr (instr_size_1) ge f i rs1 m1 = Next rs2 m2 ->
+        real_asm_inv (State rs1 m1) ->
+        real_asm_inv (State rs2 m2).
+    Proof.
+      intros f i rs1 m1 rs2 m2 NORSP INVAR EI RAI; inv RAI.
+      erewrite exec_instr_invar_same in EI; eauto.
+      erewrite <- exec_instr_invar_same' in EI; eauto.
+      exploit NORSP; eauto. intro EQ.
+      generalize (asm_prog_unchange_sup i INVAR _ _ _ _ _ _ EI). intros (A & B).
+      constructor.
+      + red in RSPPTR; red. simpl in *; rewrite <- EQ. eauto.
+      + red in BSTACKPERM; red. simpl in *. setoid_rewrite <- B. eauto.
+      + red in STOP; red; simpl in *. rewrite <- A; eauto.
+    Qed.
+
+    Lemma align_Mptr_sub:
+      forall o,
+        (align_chunk Mptr | Ptrofs.unsigned o) ->
+        (align_chunk Mptr | Ptrofs.unsigned (Ptrofs.add o (Ptrofs.neg (Ptrofs.repr (size_chunk Mptr))))).
+    Proof.
+      intros.
+      apply div_ptr_add; auto.
+      apply div_unsigned_repr.
+      apply Z.divide_opp_r.
+      apply div_unsigned_repr.
+      apply align_size_chunk_divides.
+      apply align_Mptr_modulus.
+      apply align_Mptr_modulus.
+      apply align_Mptr_modulus.
+    Qed.
+
+    Lemma align_Mptr_add:
+      forall o,
+        (align_chunk Mptr | Ptrofs.unsigned o) ->
+        (align_chunk Mptr | Ptrofs.unsigned (Ptrofs.add o (Ptrofs.repr (size_chunk Mptr)))).
+    Proof.
+      intros.
+      apply div_ptr_add; auto.
+      apply div_unsigned_repr.
+      apply align_size_chunk_divides.
+      apply align_Mptr_modulus.
+      apply align_Mptr_modulus.
+    Qed.
+
+    Lemma align_Mptr_add_gen:
+      forall o d,
+        (align_chunk Mptr | Ptrofs.unsigned o) ->
+        (align_chunk Mptr | Ptrofs.unsigned d) ->
+        (align_chunk Mptr | Ptrofs.unsigned (Ptrofs.add o d)).
+    Proof.
+      intros.
+      apply div_ptr_add; auto.
+      apply align_Mptr_modulus.
+    Qed.
+
+    Definition asm_prog_no_rsp (ge: Genv.t Asm.fundef unit):=
+      forall b f,
+        Genv.find_funct_ptr ge b = Some (Internal f) ->
+        asm_code_no_rsp (fn_code f).
+
+  Definition wf_asm_prog (ge: Genv.t Asm.fundef unit):=
+      forall b f,
+        Genv.find_funct_ptr ge b = Some (Internal f) ->
+        wf_asm_function instr_size_1 f.
+
+(*Lemma nextinstr_nf_pc: forall rs sz, nextinstr_nf rs sz PC = Val.offset_ptr (rs PC) sz.
+Proof.
+  unfold nextinstr_nf. simpl.
+  intros. f_equalrewrite Asmgenproof0.nextinstr_pc. f_equal.
+Qed. *)
+
+Lemma nextinstr_rsp:
+  forall rs sz,
+    nextinstr rs sz RSP= rs RSP.
+Proof.
+  unfold nextinstr.
+  intros; rewrite Pregmap.gso; congruence.
+Qed.
+
+Lemma nextinstr_nf_rsp:
+  forall rs sz,
+    nextinstr_nf rs sz RSP = rs RSP.
+Proof.
+  unfold nextinstr_nf.
+  intros. rewrite nextinstr_rsp.
+  rewrite Asmgenproof0.undef_regs_other; auto.
+  simpl; intuition subst; congruence.
+Qed.
+
+    Lemma real_asm_inv_inv:
+      forall (prog_no_rsp: asm_prog_no_rsp ge) (WF: wf_asm_prog ge) s1 t s2,
+        (step instr_size_1) ge s1 t s2 ->
+        real_asm_inv s1 ->
+        real_asm_inv s2.
+    Proof.
+      intros prog_no_rsp WF s1 t s2 STEP INV; inv STEP.
+      - destruct (stk_unrelated_instr i) eqn:INVAR.
+        eapply exec_instr_invar_inv; eauto.
+        eapply prog_no_rsp; eauto. eapply Asmgenproof0.find_instr_in; eauto.
+        destruct i; simpl in INVAR; try congruence.
+        + (* call_s *)
+          simpl in H2. destr_in H2. inv H2. inv INV; constructor; simpl.
+          * red. simpl. simpl_regs. destruct RSPPTR as (o & EQ & AL); simpl in *; rewrite EQ.
+            simpl. eexists; split; eauto. apply align_Mptr_sub; auto.
+          * red in BSTACKPERM; red; simpl in *.
+            intros o k p. erewrite storev_perm; eauto. intro. erewrite storev_perm; eauto.
+          * red in STOP; red; simpl in *. erewrite <- Mem.support_storev; eauto.
+        + (* call_r *)
+          simpl in H2. destr_in H2. inv H2. inv INV; constructor; simpl.
+          * red. simpl. simpl_regs. destruct RSPPTR as (o & EQ & AL); simpl in *; rewrite EQ.
+            simpl. eexists; split; eauto. apply align_Mptr_sub; auto.
+          * red in BSTACKPERM; red; simpl in *.
+            intros o k p. erewrite storev_perm; eauto. intro. erewrite storev_perm; eauto.
+          * red in STOP; red; simpl in *. erewrite <- Mem.support_storev; eauto.
+        + (* ret *)
+          simpl in H2; repeat destr_in H2; inv INV; constructor; simpl.
+          * red. simpl. simpl_regs. destruct RSPPTR as (o & EQ & AL); simpl in *; rewrite EQ.
+            simpl. eexists; split; eauto. apply align_Mptr_add; auto.
+          * red in BSTACKPERM; red; simpl in *.
+            intros o k p. eauto.
+          * red in STOP; red; simpl in *. eauto.
+        + (* allocframe *)
+          simpl in H2; repeat destr_in H2; inv INV; constructor; simpl.
+          * red. simpl.
+            (* simpl_regs. *)
+
+            unfold nextinstr. rewrite Pregmap.gso. rewrite Pregmap.gss.
+            destruct RSPPTR as (o & EQ & AL); simpl in *; rewrite EQ.
+            simpl. eexists; split; eauto. apply align_Mptr_add_gen; auto.
+            unfold Ptrofs.neg. apply div_unsigned_repr; auto. apply Z.divide_opp_r.
+            unfold Ptrofs.sub. apply div_unsigned_repr; auto.
+            apply Z.divide_sub_r.
+            apply div_unsigned_repr; auto.
+            transitivity 8. unfold Mptr. destr; simpl. exists 1; lia. exists 2; lia. apply align_divides. lia.
+            apply align_Mptr_modulus.
+            apply div_unsigned_repr; auto.
+            apply align_size_chunk_divides.
+            apply align_Mptr_modulus.
+            apply align_Mptr_modulus.
+            apply align_Mptr_modulus. congruence.
+          * red in BSTACKPERM; red; simpl in *.
+            intros o k p. erewrite storev_perm; eauto. intro. erewrite storev_perm; eauto.
+          * red in STOP; red; simpl in *. erewrite <- Mem.support_storev; eauto.
+        + (* freeframe *)
+          simpl in H2; repeat destr_in H2; inv INV; constructor; simpl.
+          * red. simpl.
+            unfold nextinstr. rewrite Pregmap.gso. rewrite Pregmap.gss.
+            (* simpl_regs. *)
+            destruct RSPPTR as (o & EQ & AL); simpl in *; rewrite EQ.
+            simpl. eexists; split; eauto. apply align_Mptr_add_gen; auto.
+            unfold Ptrofs.sub. apply div_unsigned_repr; auto.
+            apply Z.divide_sub_r.
+            apply div_unsigned_repr; auto.
+            transitivity 8. unfold Mptr. destr; simpl. exists 1; lia. exists 2; lia. apply align_divides. lia.
+            apply align_Mptr_modulus.
+            apply div_unsigned_repr; auto.
+            apply align_size_chunk_divides.
+            apply align_Mptr_modulus.
+            apply align_Mptr_modulus. congruence.
+          * red in BSTACKPERM; red; eauto.
+          * red in STOP; red; eauto.
+      - inv INV; constructor.
+        + red in RSPPTR; red; simpl in *. unfold nextinstr_nf.
+          (* repeat simpl_regs. *) rewrite nextinstr_rsp.
+          rewrite Asmgenproof0.undef_regs_other.
+          2: simpl; intuition subst; congruence.
+          exploit wf_asm_builtin_not_PC; eauto.
+          intros (NPC & NRSP & NRA).
+          rewrite set_res_other; auto.
+          rewrite Asmgenproof0.undef_regs_other.
+          eauto. setoid_rewrite in_map_iff. intros r' (x & PREG & IN). subst.
+          intro EQ. symmetry in EQ. apply preg_of_not_rsp in EQ. congruence.
+        + red in BSTACKPERM; red. simpl in *. intros o k p.
+          repeat erewrite (external_perm_stack _ _ _ _ _ _ _ _ _ _ _ H3); eauto.
+           simpl. auto. red in STOP; simpl in STOP. unfold bstack. unfold stkblock.
+           simpl. destruct STOP as (tl & st & STOP). rewrite STOP. split. auto. left. auto.
+           simpl. auto. red in STOP; simpl in STOP. unfold bstack. unfold stkblock.
+           simpl. destruct STOP as (tl & st & STOP). rewrite STOP. split. auto. left. auto.
+        + red in STOP; red; simpl in *. destruct STOP as (tl & st & STOP).
+          exploit external_call_stack; eauto. destr. intros.
+          rewrite STOP in H4. simpl in H4. destruct st. eauto. eauto.
+          intros. rewrite H4. eauto.
+      - inv INV; constructor.
+        + Opaque destroyed_at_call.
+          red in RSPPTR; red; simpl in *. repeat simpl_regs.
+          destruct RSPPTR as (o & EQ & AL); simpl in *. rewrite EQ.
+          simpl. eexists; split; eauto. apply align_Mptr_add; auto.
+        + red in BSTACKPERM; red. simpl in *. intros o k p.
+          repeat erewrite (external_perm_stack _ _ _ _ _ _ _ _ _ _ _ H2); eauto.
+           simpl. auto. red in STOP; simpl in STOP. unfold bstack. unfold stkblock.
+           simpl. destruct STOP as (tl & st & STOP). rewrite STOP. split. auto. left. auto.
+           simpl. auto. red in STOP; simpl in STOP. unfold bstack. unfold stkblock.
+           simpl. destruct STOP as (tl & st & STOP). rewrite STOP. split. auto. left. auto.
+        + red in STOP; red; simpl in *. destruct STOP as (tl & st & STOP).
+          exploit external_call_stack; eauto. destr. intros.
+          rewrite STOP in H3. simpl in H3. destruct st. eauto. eauto.
+          intros. rewrite H3. eauto.
+    Qed.
+
+End INVARIANT.
+
